rewrite: fol

src/FOL/fol.lean
@@ -1,4 +1,4 @@
-import lib.lib tactic data.set_like.basic logic
+import lib.lib tactic data.set_like.basic logic translation
 
 universe u
 
@@ -22,47 +22,39 @@ class has_mem_symbol (L : language) := (mem : L.pr 2)
 
 variables (L : language.{u})
 
-inductive term : Type u
-| var {} : ℕ → term
-| app    : ∀ {n : ℕ}, L.fn n → (fin n → term) → term
+inductive subterm (m n : ℕ) : Type u
+| metavar {} : fin m → subterm
+| var     {} : fin n → subterm
+| function   : ∀ {p}, L.fn p → (fin p → subterm) → subterm
+
+@[reducible] def term (m) := subterm L m 0
 
 variables {L}
 
-prefix `#`:max := term.var
+namespace subterm
+variables {m n : ℕ}
 
-notation `❨` c `❩ ` v :84 := term.app c v
+prefix `#`:max := subterm.var
+prefix `&`:max := subterm.metavar
 
-def term.const (f : L.fn 0) : term L := term.app f finitary.nil
+def term.const (f : L.fn 0) : subterm L m n := function f finitary.nil
 
-instance : inhabited (term L) := ⟨#0⟩
+instance [inhabited (fin m)] : inhabited (subterm L m n) := ⟨&default⟩
 
-instance [has_zero_symbol L] : has_zero (term L) := ⟨term.app has_zero_symbol.zero finitary.nil⟩
+instance [has_zero_symbol L] : has_zero (subterm L m n) := ⟨function has_zero_symbol.zero finitary.nil⟩
 
-instance [has_succ_symbol L] : has_succ (term L) := ⟨λ t, term.app has_succ_symbol.succ ‹t›⟩
+instance [has_succ_symbol L] : has_succ (subterm L m n) := ⟨λ t, function has_succ_symbol.succ ‹t›⟩
 
-instance [has_add_symbol L] : has_add (term L) := ⟨λ t u, term.app has_add_symbol.add ‹t, u›⟩
+instance [has_add_symbol L] : has_add (subterm L m n) := ⟨λ t u, function has_add_symbol.add ‹t, u›⟩
 
-instance [has_mul_symbol L] : has_mul (term L) := ⟨λ t u, term.app has_mul_symbol.mul ‹t, u›⟩
+instance [has_mul_symbol L] : has_mul (subterm L m n) := ⟨λ t u, function has_mul_symbol.mul ‹t, u›⟩
 
 postfix `˙`:max := numeral
 
-@[reducible] def idvar (n : ℕ) : finitary (term L) n := λ i, #i
-
-notation `##` := idvar _
-
-@[simp] lemma idvar_app (n : ℕ) (i : fin n) : (## : finitary (term L) n) i = #i := rfl
-
-@[simp] lemma idvar_eq_nil : (## : finitary (term L) 0) = finitary.nil := by ext
-
-@[simp] lemma idvar_eq_singleton : (## : finitary (term L) 1) = ‹#0› := by ext; by simp
-
-@[simp] lemma idvar_eq_doubleton : (## : finitary (term L) 2) = ‹#0, #1› := by ext; by simp
-
-@[reducible] def idvar_inv (n : ℕ) : finitary (term L) n := λ i, #(n - i - 1)
-
+/-
 notation `##'` := idvar_inv _
 
-@[simp] lemma idvar_inv_app (n : ℕ) (i : fin n) : (##' : finitary (term L) n) i = #(n - i - 1) := rfl
+@[simp] lemma idvar_inv_function (n : ℕ) (i : fin n) : (##' : finitary (term L) n) i = #(n - i - 1) := rfl
 
 @[simp] lemma idvar_inv_nil : (##' : finitary (term L) 0) = finitary.nil := by ext
 
@@ -72,40 +64,42 @@ notation `##'` := idvar_inv _
 
 variables (L)
 
-def term_to_string [∀ n, has_to_string (L.fn n)] : term L → string
-| #n := "#" ++ has_to_string.to_string n
-| (@term.app _ 0 c v) := has_to_string.to_string c
-| (@term.app _ 1 c v) := has_to_string.to_string c ++ "(" ++ term_to_string (v 0) ++ ")"
-| (@term.app _ 2 c v) := term_to_string (v 0) ++ has_to_string.to_string c ++ term_to_string (v 1)
-| (@term.app _ (n + 3) c v) :=
-    has_to_string.to_string c ++ "(" ++ @has_to_string.to_string (finitary _ _) _ (λ i, term_to_string (v i)) ++ ")"
 
-instance [∀ n, has_to_string (L.fn n)] : has_to_string (term L) := ⟨term_to_string L⟩
+-/
 
-inductive formula : Type u
-| verum : formula
-| app   : ∀ {n : ℕ}, L.pr n → (fin n → term L) → formula
-| equal : term L → term L → formula
-| imply : formula → formula → formula
-| neg   : formula → formula
-| fal   : formula → formula
+variables (L) (m n)
 
-notation `❴` c `❵` := formula.app c
+end subterm
 
-instance [has_le_symbol L] : has_preceq (term L) (formula L) := ⟨λ t u, formula.app has_le_symbol.le ‹t, u›⟩
-
-instance [has_mem_symbol L] : has_elem (term L) (formula L) := ⟨λ t u, formula.app has_mem_symbol.mem ‹t, u›⟩
+variables (L)
+inductive subformula (m) : ℕ → Type u
+| verum    {n} : subformula n
+| relation {n} : ∀ {p}, L.pr p → (fin p → subterm L m n) → subformula n
+| equal    {n} : subterm L m n  → subterm L m n → subformula n
+| imply    {n} : subformula n → subformula n → subformula n
+| neg      {n} : subformula n → subformula n
+| fal      {n} : subformula (n + 1) → subformula n
 
 attribute [pattern]  has_eq.eq has_negation.neg has_arrow.arrow has_univ_quantifier.univ has_exists_quantifier.ex
 
-namespace formula
-variables {L}
+@[reducible] def formula (m) := subformula L m 0
 
-def and (p : formula L) (q : formula L) : formula L := (p.imply q.neg).neg
+@[reducible] def sentence := formula L 0
 
-def or (p : formula L) (q : formula L) : formula L := p.neg.imply q
+namespace subformula
+variables {L} {m n : ℕ}
 
-instance : has_logic_symbol (formula L) :=
+instance [has_le_symbol L] : has_preceq (subterm L m n) (subformula L m n) := ⟨λ t u, relation has_le_symbol.le ‹t, u›⟩
+
+instance [has_mem_symbol L] : has_elem (subterm L m n) (subformula L m n) := ⟨λ t u, relation has_mem_symbol.mem ‹t, u›⟩
+
+def and (p : subformula L m n) (q : subformula L m n) : subformula L m n := (p.imply q.neg).neg
+
+def or (p : subformula L m n) (q : subformula L m n) : subformula L m n := p.neg.imply q
+
+def ex (p : subformula L m (n + 1)) : subformula L m n := p.neg.fal.neg
+
+instance : has_logic_symbol (subformula L m n) :=
 { bot := verum.neg,
   top := verum,
   sup := or,
@@ -113,1341 +107,505 @@ instance : has_logic_symbol (formula L) :=
   arrow := imply,
   neg := neg }
 
-instance : has_eq (term L) (formula L) := ⟨formula.equal⟩
+instance : inhabited (subformula L m n) := ⟨⊤⟩
 
-instance : has_univ_quantifier (formula L) := ⟨formula.fal⟩
+instance : has_eq (subterm L m n) (subformula L m n) := ⟨equal⟩
 
-end formula
+instance : has_univ_quantifier' (subformula L m) := ⟨@fal L m⟩
 
-def formula_to_string [has_to_string (term L)] [∀ n, has_to_string (L.pr n)] : formula L → string
-| ⊤                      := "⊤"
-| (@formula.app _ 0 p v) := has_to_string.to_string p
-| (@formula.app _ 1 p v) := has_to_string.to_string p ++ "(" ++ has_to_string.to_string (v 0) ++ ")"
-| (@formula.app _ 2 p v) := has_to_string.to_string (v 0) ++ has_to_string.to_string p ++ has_to_string.to_string (v 1)
-| (@formula.app _ (n + 3) p v) :=
-    has_to_string.to_string p ++ "(" ++ @has_to_string.to_string (finitary _ _) _ v ++ ")"
-| (t ≃ u) := has_to_string.to_string t ++ " = " ++ has_to_string.to_string u
-| (p ⟶ q) := formula_to_string p ++ " → " ++ formula_to_string q
-| (∼p) := "¬(" ++ formula_to_string p ++ ")"
-| (∀.p) := "∀(" ++ formula_to_string p ++ ")"
+instance : has_exists_quantifier' (subformula L m) := ⟨@ex L m⟩
 
-instance [has_to_string (term L)] [∀ n, has_to_string (L.pr n)] : has_to_string (formula L) := ⟨formula_to_string L⟩
+lemma top_eq : @subformula.verum L m n = (⊤) := rfl
+lemma imply_eq : @subformula.imply L m n = (⟶) := rfl
+lemma equal_eq : @subformula.equal L m n = (=') := rfl
+lemma neg_eq : @subformula.neg L m n = has_negation.neg := rfl
+lemma fal_eq : @subformula.fal L m n = has_univ_quantifier'.univ := rfl
 
-@[simp] lemma formula.top_eq : @formula.verum L = (⊤) := rfl
-@[simp] lemma formula.imply_eq : @formula.imply L = (⟶) := rfl
-@[simp] lemma formula.equal_eq : @formula.equal L = (≃) := rfl
-@[simp] lemma formula.neg_eq : @formula.neg L = has_negation.neg := rfl
-@[simp] lemma formula.fal_eq : @formula.fal L = has_univ_quantifier.univ := rfl
+lemma ex_def (p : subformula L m (n + 1)) : ∃'p = ∼∀'∼p := rfl
 
-instance : inhabited (formula L) := ⟨(#0 : term L) ≃ #0⟩
+lemma bot_def : (⊥ : subformula L m n) = ∼⊤ := rfl
 
-@[reducible] def Theory (L : language.{u}) := logic.Theory (formula L)
+@[simp] lemma equal.inj' (t₁ u₁ t₂ u₂ : subterm L m n) : (t₁ =' t₂ : subformula L m n) = (u₁ =' u₂) ↔ t₁ = u₁ ∧ t₂ = u₂ :=
+⟨equal.inj, by simp; exact congr_arg2 (=')⟩
 
-variables {L}
+@[simp] lemma imply.inj' (p₁ q₁ p₂ q₂ : subformula L m n) : p₁ ⟶ p₂ = q₁ ⟶ q₂ ↔ p₁ = q₁ ∧ p₂ = q₂ :=
+⟨imply.inj, by simp; exact congr_arg2 (⟶)⟩
 
-def formula.ex (p : formula L) : formula L := ∼∀.∼p
+@[simp] lemma neg.inj' (p q : subformula L m n) : ∼p = ∼q ↔ p = q := ⟨neg.inj, congr_arg _⟩
 
-instance : has_exists_quantifier (formula L) := ⟨formula.ex⟩
+@[simp] lemma and.inj' (p₁ q₁ p₂ q₂ : subformula L m n) : p₁ ⊓ p₂ = q₁ ⊓ q₂ ↔ p₁ = q₁ ∧ p₂ = q₂ :=
+by simp[has_inf.inf, and]
 
-lemma formula.ex_eq (p : formula L) : (∃. p) = ∼∀.∼p := rfl
+@[simp] lemma or.inj' (p₁ q₁ p₂ q₂ : subformula L m n) : p₁ ⊔ p₂ = q₁ ⊔ q₂ ↔ p₁ = q₁ ∧ p₂ = q₂ :=
+by simp[has_sup.sup, or]
 
-@[simp] lemma formula.equal.inj' (t₁ u₁ t₂ u₂ : term L) : (t₁ ≃ t₂ : formula L) = (u₁ ≃ u₂) ↔ t₁ = u₁ ∧ t₂ = u₂ :=
-⟨formula.equal.inj, by simp; exact congr_arg2 (≃)⟩
+@[simp] lemma fal.inj' (p q : subformula L m (n + 1)) : (∀'p : subformula L m n) = ∀'q ↔ p = q := ⟨fal.inj, congr_arg _⟩
 
-@[simp] lemma formula.imply.inj' (p₁ q₁ p₂ q₂ : formula L) : p₁ ⟶ p₂ = q₁ ⟶ q₂ ↔ p₁ = q₁ ∧ p₂ = q₂ :=
-⟨formula.imply.inj, by simp; exact congr_arg2 (⟶)⟩
+@[simp] lemma ex.inj' (p q : subformula L m (n + 1)) : (∃'p : subformula L m n) = ∃'q ↔ p = q := 
+by simp[has_exists_quantifier'.ex, ex]
 
-@[simp] lemma formula.neg.inj' (p q : formula L) : ∼p = ∼q ↔ p = q := ⟨formula.neg.inj, congr_arg _⟩
+end subformula
 
-@[simp] lemma formula.and.inj' (p₁ q₁ p₂ q₂ : formula L) : p₁ ⊓ p₂ = q₁ ⊓ q₂ ↔ p₁ = q₁ ∧ p₂ = q₂ :=
-by {simp[has_inf.inf, formula.and],}
+@[reducible] def preTheory (L : language.{u}) (m : ℕ) := logic.Theory (subformula L m 0)
 
-@[simp] lemma formula.or.inj' (p₁ q₁ p₂ q₂ : formula L) : p₁ ⊔ p₂ = q₁ ⊔ q₂ ↔ p₁ = q₁ ∧ p₂ = q₂ :=
-by simp[has_sup.sup, formula.or]
+@[reducible] def Theory (L : language.{u}) := logic.Theory (subformula L 0 0)
 
-@[simp] lemma formula.fal.inj' (p q : formula L) : (∀.p : formula L) = ∀.q ↔ p = q := ⟨formula.fal.inj, congr_arg _⟩
+namespace subterm
 
-@[simp] lemma formula.ex.inj' (p q : formula L) : (∃. p : formula L) = ∃. q ↔ p = q := 
-by simp[has_exists_quantifier.ex, formula.ex]
+section rew
+variables {L} {m m₁ m₂ m₃ n : ℕ}
 
-@[simp] lemma formula.verum_ne_predicate {n} (r : L.pr n) (v : finitary (term L) n) :
-  (⊤ : formula L) ≠ formula.app r v.
+@[simp] def rew (s : finitary (subterm L m₂ n) m₁) : subterm L m₁ n → subterm L m₂ n
+| (&x)           := s x
+| (#x)           := #x
+| (function f v) := function f (λ i, (v i).rew)
 
-@[simp] lemma formula.verum_ne_equal (t u : term L) : (⊤ : formula L) ≠ (t ≃ u).
+section rew
 
-@[simp] lemma formula.verum_ne_imply (p q : formula L) : ⊤ ≠ (p ⟶ q).
+lemma eq_rew_of_eq {t : subterm L m₁ n} {s₁ s₂ : finitary (subterm L m₂ n) m₁} (h : s₁ = s₂) :
+  rew s₁ t = rew s₂ t := by rw[h]
 
-@[simp] lemma formula.verum_ne_neg (p : formula L) : ⊤ ≠ ∼p.
+lemma nested_rew {m₁ m₂ m₃} (s₀ : finitary (subterm L m₂ n) m₁) (s₁ : finitary (subterm L m₃ n) m₂) :
+  ∀ t, rew s₁ (rew s₀ t) = rew (rew s₁ ∘ s₀) t
+| (&x)           := by simp
+| (#x)           := by simp
+| (function f v) := by simp; funext i; exact nested_rew (v i)
 
-@[simp] lemma formula.verum_ne_fal (p : formula L) : ⊤ ≠ ∀.p.
+@[simp] lemma rew_metavar (t : subterm L m n) : rew metavar t = t :=
+by induction t; simp*
 
-@[simp] lemma formula.predicate_ne_verum {n} (r : L.pr n) (v : finitary (term L) n) :
-  formula.app r v ≠ ⊤.
+end rew
 
-@[simp] lemma formula.predicate_ne_equal {n} (r : L.pr n) (v : finitary (term L) n) (t u : term L) :
-  formula.app r v ≠ (t ≃ u).
+def subst (t : subterm L m n) : subterm L (m + 1) n → subterm L m n :=
+rew (@fin.cases m (λ _, subterm L m n) t metavar) 
 
-@[simp] lemma formula.predicate_ne_imply {n} (r : L.pr n) (v : finitary (term L) n) (p q : formula L) :
-  formula.app r v ≠ p ⟶ q.
+section subst
 
-@[simp] lemma formula.predicate_ne_neg {n} (r : L.pr n) (v : finitary (term L) n) (p : formula L) :
-  formula.app r v ≠ ∼p.
+@[simp] lemma subst_var (u : subterm L m n) (x) : subst u #x = #x := rfl
 
-@[simp] lemma formula.predicate_ne_fal {n} (r : L.pr n) (v : finitary (term L) n) (p : formula L) :
-  formula.app r v ≠ ∀.p.
+@[simp] lemma subst_metavar_zero (u : subterm L m n) : subst u &0 = u := rfl
 
-@[simp] lemma formula.equal_ne_verum (t u : term L) :
-  (t ≃ u : formula L) ≠ ⊤.
+@[simp] lemma subst_metavar_succ (u : subterm L m n) (x : fin m) : subst u &x.succ = &x := by simp[subst]
 
-@[simp] lemma formula.equal_ne_predivate (t u : term L) {n} (r : L.pr n) (v : finitary (term L) n) :
-  (t ≃ u) ≠ formula.app r v.
+@[simp] lemma subst_function (u : subterm L m n) {p} (f : L.fn p) (v) : subst u (function f v) = function f (subst u ∘ v) := by simp[subst]
 
-@[simp] lemma formula.equal_ne_imply (t u : term L) (p q : formula L) :
-  (t ≃ u) ≠ p ⟶ q.
+end subst
 
-@[simp] lemma formula.equal_ne_neg (t u : term L) (p : formula L) :
-  (t ≃ u) ≠ ∼p.
+def mlift' : subterm L m n → subterm L (m + 1) n := rew (metavar ∘ fin.succ)
 
-@[simp] lemma formula.equal_ne_fal (t u : term L) (p : formula L) :
-  (t ≃ u : formula L) ≠ ∀.p.
+@[simp] def lift : subterm L m n → subterm L m (n + 1)
+| (#x)           := #x.succ
+| (&x)           := &x
+| (function f v) := function f (λ i, (v i).lift)
 
-@[simp] lemma formula.imply_ne_verum (p q : formula L) :
-  p ⟶ q ≠ ⊤.
+section lift
 
-@[simp] lemma formula.imply_ne_predicate (p q : formula L) {n} (r : L.pr n) (v : finitary (term L) n) :
-  p ⟶ q ≠ formula.app r v.
+lemma lift_rew (s : finitary (subterm L m₂ n) m₁) (t : subterm L m₁ n) : (t.rew s).lift = t.lift.rew (lift ∘ s) :=
+by induction t with x x p f v IH; simp; exact funext IH
 
-@[simp] lemma formula.imply_ne_equal (p q : formula L) (t u : term L) :
-  p ⟶ q ≠ (t ≃ u).
+end lift
 
-@[simp] lemma formula.imply_ne_neg (p q r : formula L) : p ⟶ q ≠ ∼r.
+@[simp] def mlift : subterm L m n → subterm L (m + 1) n
+| (&x)           := &x.succ
+| (#x)           := #x
+| (function f v) := function f (λ i, (v i).mlift)
 
-@[simp] lemma formula.imply_ne_fal (p q r : formula L) : p ⟶ q ≠ ∀.r.
+section mlift
 
-@[simp] lemma formula.neg_ne_verum (p : formula L) : ∼p ≠ ⊤.
+lemma mlift_eq_rew : @mlift L m n = rew (metavar ∘ fin.succ) :=
+funext (λ t, by induction t; simp*)
 
-@[simp] lemma formula.neg_ne_predicate (p : formula L) {n} (r : L.pr n) (v : finitary (term L) n) :
- ∼p ≠ formula.app r v.
+lemma mlift_rew (s : finitary (subterm L m₂ n) m₁) (t : subterm L m₁ n) : (t.rew s).mlift = t.rew (mlift ∘ s) :=
+by induction t with x x p f v IH; simp; exact funext IH
 
-@[simp] lemma formula.neg_ne_equal (p : formula L) (t u : term L) : ∼p ≠ (t ≃ u).
+lemma mlift_lift (t : subterm L m n) : t.lift.mlift = t.mlift.lift :=
+by induction t; simp*
 
-@[simp] lemma formula.neg_ne_imply (p q r : formula L) : ∼p ≠ (q ⟶ r).
+@[simp] lemma subst_mlift (u : subterm L m n) (t : subterm L m n) :
+  subst u t.mlift = t :=
+by induction t; simp; exact funext (λ x, by simp*)
 
-@[simp] lemma formula.neg_ne_fal (p q : formula L) : ∼p ≠ ∀.q.
+lemma mlift_subst (u : subterm L m n) (t : subterm L (m + 1) n) :
+  (subst u t).mlift = t.rew (@fin.cases m (λ _, subterm L (m + 1) n) (mlift u) (mlift ∘ metavar)) :=
+by simp[subst, mlift_rew];
+   refine eq_rew_of_eq (funext $ λ x, by rcases (fin.eq_zero_or_eq_succ x) with (rfl | ⟨x, rfl⟩); simp) 
 
-@[simp] lemma formula.fal_ne_verum (p : formula L) :
-  ∀.p ≠ ⊤.
+end mlift
 
-@[simp] lemma formula.fal_ne_predicate (p : formula L) {n} (r : L.pr n) (v : finitary (term L) n) :
-  ∀.p ≠ formula.app r v.
+/-
+  #0 #1 #2 #3 #4 ... #(n - 1) #n &0 &1 &3 &4 ... &(m - 1)
+      ↓push                       ↑pull
+  #0 #1 #2 #3 #4 ... #(n - 1) &0 &1 &3 &4 &5 ... &m
+-/
 
-@[simp] lemma formula.fal_ne_equal (p : formula L) (t u : term L) :
-  (∀.p : formula L) ≠ (t ≃ u).
+def push : subterm L m (n + 1) → subterm L (m + 1) n
+| (&x)           := &x.succ
+| (#x)           := @fin.last_cases n (λ _, subterm L (m + 1) n) &0 var x
+| (function f v) := function f (λ i, (v i).push)
 
-@[simp] lemma formula.fal_ne_imp (p q r : formula L) : (∀.p : formula L) ≠ (q ⟶ r).
+section push
 
-@[simp] lemma formula.fal_ne_neg (p q : formula L) : (∀.p : formula L) ≠ ∼q.
+@[simp] lemma push_metavar (x) : (&x : subterm L m (n + 1)).push = &x.succ := rfl
 
-@[simp] lemma formula.fal_ne_ex (p q : formula L) : (∀.p : formula L) ≠ ∃. q.
+@[simp] lemma push_var_zero_last : (#(fin.last n) : subterm L m (n + 1)).push = &0 := by simp[push]
 
-@[simp] lemma formula.ex_ne_fal (p q : formula L) : (∃. p : formula L) ≠ ∀.q.
+@[simp] lemma push_var_zero (x) : (#(fin.cast_succ x) : subterm L m (n + 1)).push = #x := by simp[push]
 
-@[simp] def nfal (p : formula L) : ℕ → formula L
-| 0     := p
-| (n+1) := ∀.(nfal n)
+@[simp] lemma push_function {p} (f : L.fn p) (v : fin p → subterm L m (n + 1)) :
+  (function f v : subterm L m (n + 1)).push = function f (push ∘ v) := by simp[push]
 
-notation `∀.[` i `] `:90 p := nfal p i
+end push
 
-@[simp] def nex (p : formula L) : ℕ → formula L
-| 0     := p
-| (n+1) := ∃. (nex n)
+def pull : subterm L (m + 1) n → subterm L m (n + 1)
+| (&x)           := fin.cases #(fin.last n) metavar x
+| (#x)           := #x.cast_succ
+| (function f v) := function f (λ i, (v i).pull)
 
-notation `∃.[` i `] `:90 p := nex p i
+section pull
 
-@[simp] lemma nfal_fal (p : formula L) (i : ℕ) : (∀.[i] (∀.p)) = ∀.(∀.[i] p) :=
-by { induction i with i IH; simp, exact IH }
+@[simp] lemma pull_metavar_zero : (&0 : subterm L (m + 1) n).pull = #(fin.last n) := rfl
 
-@[simp] lemma nex_ex (p : formula L) (i : ℕ) : (∃.[i] (∃. p)) = ∃. (∃.[i] p) :=
-by { induction i with i IH; simp, exact IH }
+@[simp] lemma pull_metavar_succ (x : fin m) : (&x.succ : subterm L (m + 1) n).pull = &x := by simp[pull]
 
-notation `ı` := term.var
+@[simp] lemma pull_var (x) : (#x : subterm L (m + 1) n).pull = #x.cast_succ := by simp[pull]
 
-def slide {α : Type*} (s : ℕ → α) (a : α) (n : ℕ) : ℕ → α :=
-λ x, if x < n then s x else if n < x then s (x - 1) else a
-notation s `[`:1200 n ` ⇝ `:95 t `]`:0 := slide s t n
+@[simp] lemma pull_function {p} (f : L.fn p) (v : fin p → subterm L (m + 1) n) :
+  (function f v : subterm L (m + 1) n).pull = function f (pull ∘ v) := by simp[pull]
 
-@[simp] lemma slide_eq {α : Type*} (s : ℕ → α) (a : α) (n) : s[n ⇝ a] n = a := by simp[slide]
+@[simp] lemma push_pull (t : subterm L m (n + 1)) : t.push.pull = t :=
+by{ induction t, 
+    case metavar : x { simp },
+    case var : x { refine fin.last_cases _ _ x; simp },
+    case function : p f v IH { simp, funext x, simp[IH] } }
 
-@[simp] lemma slide_lt {α : Type*} (s : ℕ → α) (a : α) (n m) (h : m < n) : s[n ⇝ a] m = s m := by simp[slide, h]
+@[simp] lemma pull_push (t : subterm L (m + 1) n) : t.pull.push = t :=
+by{ induction t,
+    case metavar : x { refine fin.cases _ _ x; simp },
+    case var : x { simp },
+    case function : p f v IH { simp, funext x, simp[IH] } }
 
-@[simp] lemma slide_gt {α : Type*} (s : ℕ → α) (a : α) (n m) (h : n < m) : s[n ⇝ a] m = s (m - 1) :=
-by {simp[slide, h], intros hh, exfalso, exact nat.lt_asymm h hh }
+end pull
 
-def concat {α : Type*} (s : ℕ → α) (a : α) : ℕ → α := s [0 ⇝ a]
-notation a ` ⌢ `:90 s := concat s a
+def dummy : subterm L m n → subterm L m (n + 1) := pull ∘ mlift
 
-@[simp] lemma concat_0 {α : Type*} (s : ℕ → α) (a : α) : (a ⌢ s) 0 = a := rfl
-@[simp] lemma concat_succ {α : Type*} (s : ℕ → α) (a : α) (n : ℕ) :
-  (a ⌢ s) (n + 1) = s n := rfl
+section dummy
 
-lemma slide_perm (i : ℕ) (t : term L) : ∀ n, ∃ m, ı[i ⇝ t] m = #n := λ n,
-by { have C : n < i ∨ i ≤ n, exact lt_or_ge n i,
-     cases C, refine ⟨n, by simp[C]⟩, 
-     refine ⟨n + 1, _⟩, simp[nat.lt_succ_iff.mpr C] }
+@[simp] lemma dummy_metavar (x) : dummy (&x : subterm L m n) = &x := by simp[dummy]
 
-def discard {α : Type*} (s : ℕ → α) (n : ℕ) : ℕ → α :=
-λ x, if x < n then s x else s (x + 1)
+@[simp] lemma dummy_var (x) : dummy (#x : subterm L m n) = #x.cast_succ := by simp[dummy]
 
-notation s `-{`:1200 n `}`:0 := discard s n
+@[simp] lemma dummy_function {p} (f : L.fn p) (v : finitary (subterm L m n) p) :
+  dummy (function f v) = function f (dummy ∘ v) := by simp[dummy]
 
-@[simp] lemma discard_of_lt {α : Type*} (s : ℕ → α) {m n} (h : m < n) :
- s-{n} m = s m := by simp[discard, h]
+end dummy
 
-@[simp] lemma discard_of_le {α : Type*} (s : ℕ → α) {m n} (h : n ≤ m) :
- s-{n} m = s (m + 1) := by {simp[discard, h],  intros hlt, exfalso, exact nat.lt_le_antisymm hlt h }
+end rew
 
-lemma discard_0_eq_add_one {α : Type*} (s : ℕ → α) : s-{0} = λ x, s (x + 1) :=
-by funext x; simp
+end subterm
 
-namespace term
+namespace subformula
+open subterm finitary
+variables {L} {m m₁ m₂ m₃ n : ℕ}
 
-@[simp] def rew (s : ℕ → term L) : term L → term L
-| (#x)      := s x
-| (❨f❩ v) := ❨f❩ (λ i, (v i).rew)
+@[simp] def complexity : Π {n}, subformula L m n → ℕ
+| n verum          := 0
+| n (relation p v) := 0
+| n (equal t u)    := 0
+| n (imply p q)    := max p.complexity q.complexity + 1
+| n (neg p)        := p.complexity + 1
+| n (fal p)        := p.complexity + 1
 
-@[reducible] def rew_var (s : ℕ → ℕ) : term L → term L := λ t, t.rew (λ x, #(s x))
+@[simp] lemma imply_complexity (p q : subformula L m n) : (p ⟶ q).complexity = max p.complexity q.complexity + 1 := by refl
 
-@[simp] lemma constant_rew (c : L.fn 0) (s : ℕ → term L) {v : finitary (term L) 0} : (app c v).rew s = app c finitary.nil :=
-by simp
+def rew' {m₁ m₂} : Π {n}, finitary (subterm L m₂ n) m₁ → subformula L m₁ n → subformula L m₂ n
+| n s verum          := ⊤
+| n s (relation p v) := relation p (λ i, (v i).rew s)
+| n s (equal t u)    := (t.rew s) =' (u.rew s)
+| n s (imply p q)    := p.rew' s ⟶ q.rew' s
+| n s (neg p)        := ∼p.rew' s
+| n s (fal p)        := ∀'p.rew' (subterm.lift ∘ s)
 
-@[simp] lemma unary_rew (f : L.fn 1) (s : ℕ → term L) (v : finitary (term L) 1) :
-  (app f v).rew s = app f ‹(v 0).rew s› :=
-by simp; ext; simp
+def rew (s : finitary (subterm L m₂ n) m₁) : subformula L m₁ n →ₗ subformula L m₂ n :=
+{ to_fun := rew' s,
+  map_neg' := λ p, by refl,
+  map_imply' := λ p q, by refl,
+  map_and' := λ p q, by refl,
+  map_or' := λ p q, by refl,
+  map_top' := by refl,
+  map_bot' := by refl }
 
-@[simp] lemma binary_rew (f : L.fn 2) (s : ℕ → term L) (v : finitary (term L) 2) :
-  (app f v).rew s = app f ‹(v 0).rew s, (v 1).rew s› :=
-by simp; ext; simp
+section rew
+variables (s : finitary (subterm L m₂ n) m₁)
 
-@[simp] lemma zero_rew [has_zero_symbol L] (s : ℕ → term L) : (0 : term L).rew s = 0 :=
-by unfold has_zero.zero; simp
+lemma rew_def (p : subformula L m₁ n) : rew s p = rew' s p := rfl
 
-@[simp] lemma succ_rew [has_succ_symbol L] (t : term L) (s : ℕ → term L) : (Succ t : term L).rew s = Succ (t.rew s) :=
-by unfold has_succ.succ; simp; ext; simp
+variables {s}
 
-@[simp] lemma numeral_rew [has_zero_symbol L] [has_succ_symbol L] (n : ℕ) (s : ℕ → term L) :
-  (n˙ : term L).rew s = n˙ :=
-by induction n; simp[*, numeral]
+@[simp] lemma rew_relation {p} (r : L.pr p) (v) :
+  rew s (relation r v) = relation r (subterm.rew s ∘ v) := rfl
 
-@[simp] lemma add_rew [has_add_symbol L] (t u : term L) (s : ℕ → term L) : (t + u : term L).rew s = t.rew s + u.rew s :=
-by unfold has_add.add; simp; ext; simp
+@[simp] lemma rew_equal (t u : subterm L m₁ n) :
+  rew s (t =' u) = (t.rew s =' u.rew s) := rfl
 
-@[simp] lemma mul_rew [has_mul_symbol L] (t u : term L) (s : ℕ → term L) : (t * u : term L).rew s = t.rew s * u.rew s :=
-by unfold has_mul.mul; simp; ext; simp
+@[simp] lemma rew_fal (p : subformula L m₁ (n + 1)) :
+  rew s (∀'p) = ∀'rew (subterm.lift ∘ s) p := rfl
 
-instance : has_pow (term L) ℕ := ⟨λ t i, t.rew (λ x, #(x + i))⟩
+@[simp] lemma rew_ex (p : subformula L m₁ (n + 1)) :
+  rew s (∃'p) = ∃'rew (subterm.lift ∘ s) p := by simp[ex_def]
 
-instance finitary_pow {n : ℕ} : has_pow (fin n → term L) ℕ := ⟨λ v m, (λ i, (v i^m))⟩
+lemma rew_eq_self_of_eq {s : finitary (subterm L m n) m} (h : s = metavar) (p : subformula L m n) : rew s p = p :=
+by { induction p; simp[top_eq, equal_eq, imply_eq, neg_eq, fal_eq, subterm.mlift_rew, *],
+     case relation : n p r v { funext x; simp },
+     case fal : n p IH { refine IH (funext $ by simp) } }
 
-lemma pow_eq (v : term L) (i : ℕ) : v^i = v.rew (λ x, #(x + i)) := rfl
+@[simp] lemma rew_metavar (p : subformula L m n) : rew metavar p = p := rew_eq_self_of_eq rfl p
 
-@[simp] lemma finitary_pow_app {n} (v : fin n → term L) (i : fin n) (m : ℕ) : (v^m) i = (v i)^m := rfl
+lemma nested_rew {m₁ m₂ m₃} : ∀ {n} (p : subformula L m₁ n) (s₀ : finitary (subterm L m₂ n) m₁) (s₁ : finitary (subterm L m₃ n) m₂),
+  rew s₁ (rew s₀ p) = rew (subterm.rew s₁ ∘ s₀) p
+| n verum          s₀ s₁ := by simp[top_eq]
+| n (relation p v) s₀ s₁ := by simp; funext; simp[subterm.nested_rew]
+| n (equal t u)    s₀ s₁ := by simp[equal_eq, subterm.nested_rew]
+| n (imply p q)    s₀ s₁ := by simp[imply_eq, nested_rew p, nested_rew q]
+| n (neg p)        s₀ s₁ := by simp[neg_eq, nested_rew p]
+| n (fal p)        s₀ s₁ := by simp[fal_eq, nested_rew p]; { 
+  have : subterm.rew (subterm.lift ∘ s₁) ∘ subterm.lift ∘ s₀ = subterm.lift ∘ subterm.rew s₁ ∘ s₀,
+  { funext i; simp[lift_rew] },
+  rw this }
 
-@[simp] lemma var_pow (n i : ℕ) : (#n : term L)^i = #(n + i) := rfl
+lemma eq_rew_of_eq {p : subformula L m₁ n} {s₁ s₂ : finitary (subterm L m₂ n) m₁} (h : s₁ = s₂) :
+  rew s₁ p = rew s₂ p := by rw[h]
 
-@[simp] lemma app_pow {n} (f : L.fn n) (v : fin n → (term L)) (i : ℕ) : (❨f❩ v)^i = ❨f❩ (v^i) := rfl
+end rew
 
-@[simp] lemma unary_pow (f : L.fn 1) (v : finitary (term L) 1) (i : ℕ) :
-  (app f v)^ i = app f ‹(v 0)^i› :=
-by simp[pow_eq]
+def subst (t : subterm L m n) : subformula L (m + 1) n →ₗ subformula L m n :=
+rew (@fin.cases m (λ _, subterm L m n) t metavar)
 
-@[simp] lemma binary_pow(f : L.fn 2) (v : finitary (term L) 2) (i : ℕ):
-  (app f v)^i = app f ‹(v 0)^i, (v 1)^i› :=
-by simp[pow_eq]
+section subst
+variables (u : subterm L m n)
 
-@[simp] lemma zero_pow [has_zero_symbol L] (i : ℕ) : (0 : term L)^i = 0 := by simp[pow_eq]
+@[simp] lemma subst_relation {p} (r : L.pr p) (v) :
+  subst u (relation r v) = relation r (subterm.subst u ∘ v) := by simp[subst, subterm.subst]
 
-@[simp] lemma succ_pow [has_succ_symbol L] (t : term L) (i : ℕ) : (Succ t : term L)^i = Succ (t^i) :=
-by simp[pow_eq]
+@[simp] lemma subst_equal (t₁ t₂ : subterm L (m + 1) n) :
+  subst u (t₁ =' t₂) = (u.subst t₁ =' u.subst t₂) := by simp[subst, subterm.subst]
 
-@[simp] lemma numeral_pow [has_zero_symbol L] [has_succ_symbol L] (n : ℕ) (i : ℕ) :
-  (n˙ : term L)^i = n˙ :=
-by simp[pow_eq]
+@[simp] lemma subst_fal (p : subformula L (m + 1) (n + 1)) :
+  subst u (∀'p) = ∀'subst u.lift p :=
+by simp[subst]; refine eq_rew_of_eq (funext $ λ x, by rcases (fin.eq_zero_or_eq_succ x) with (rfl | ⟨x, rfl⟩); simp)
 
-@[simp] lemma add_pow [has_add_symbol L] (t u : term L) (i : ℕ) : (t + u : term L)^i = t^i + u^i :=
-by simp[pow_eq]
+@[simp] lemma subst_ex (p : subformula L (m + 1) (n + 1)) :
+  subst u (∃'p) = ∃'subst u.lift p := by simp[ex_def]
 
-@[simp] lemma mul_pow [has_mul_symbol L] (t u : term L) (i : ℕ) : (t * u : term L)^i = t^i * u^i :=
-by simp[pow_eq]
+end subst
 
-@[simp] lemma rew_var_inj_of_inj :
-  ∀ {t u : term L} {s : ℕ → ℕ} (I : function.injective s),
-  t.rew_var s = u.rew_var s ↔ t = u
-| #x               #y               s I := by { simp[rew_var], exact ⟨@I x y, congr_arg (λ (x : ℕ), s x)⟩ }
-| #x               (term.app f v)   s I := by simp[rew_var]
-| (term.app f v)   #x               s I := by simp[rew_var]
-| (term.app f₁ v₁) (term.app f₂ v₂) s I :=
-    begin
-      simp[rew_var], rintros rfl rfl, simp, split,
-      { intros h, funext j,
-        have : (v₁ j).rew_var s = (v₂ j).rew_var s,
-        { have := congr_fun h j, simp at this, exact this },
-        exact (@rew_var_inj_of_inj (v₁ j) (v₂ j) s I).mp this },
-      { rintros rfl, simp }
-    end
+def mlift' {m} : Π {n}, subformula L m n → subformula L (m + 1) n
+| n verum          := ⊤
+| n (relation p v) := relation p (mlift ∘ v)
+| n (equal t u)    := t.mlift =' u.mlift
+| n (imply p q)    := p.mlift' ⟶ q.mlift'
+| n (neg p)        := ∼p.mlift'
+| n (fal p)        := ∀'p.mlift'
 
-@[simp] lemma pow_inj : ∀ {t u : term L} {i : ℕ}, t^i = u^i ↔ t = u :=
-λ t u i, by { simp[has_pow.pow], refine rew_var_inj_of_inj (λ x y, by simp) }
+def mlift : subformula L m n →ₗ subformula L (m + 1) n :=
+{ to_fun := mlift',
+  map_neg' := λ p, by refl,
+  map_imply' := λ p q, by refl,
+  map_and' := λ p q, by refl,
+  map_or' := λ p q, by refl,
+  map_top' := by refl,
+  map_bot' := by refl }
 
-@[simp] lemma finitary_pow_inj {n} {v w : fin n → term L} {i : ℕ} : v^i = w^i ↔ v = w :=
-⟨λ h, funext (λ j, by { have := congr_fun h j, simp at this, exact this }),
-  by { rintros rfl, simp }⟩
+section mlift
 
-@[simp] def arity : term L → ℕ
-| (#n)    := n + 1
-| (❨f❩ v) := ⨆ᶠ i, (v i).arity
+@[simp] lemma mlift_relation {p} (r : L.pr p) (v : finitary (subterm L m n) p) :
+  mlift (relation r v) = relation r (subterm.mlift ∘ v) := rfl
 
-@[simp] lemma constant_arity (c : L.fn 0) {v : finitary (term L) 0} : (app c v).arity = 0 :=
-by simp
+@[simp] lemma mlift_equal (t u : subterm L m n) :
+  mlift (t =' u : subformula L m n) = (t.mlift =' u.mlift) := rfl
 
-@[simp] lemma unary_arity (f : L.fn 1) {v : finitary (term L) 1} : (❨f❩ v).arity = (v 0).arity :=
-by simp
+@[simp] lemma mlift_fal (p : subformula L m (n + 1)) :
+  mlift (∀'p) = ∀'mlift p := rfl
 
-@[simp] lemma binary_arity (f : L.fn 2) (v : finitary (term L) 2) :
-  (❨f❩ v).arity = max (v 0).arity (v 1).arity :=
-by simp
+@[simp] lemma mlift_ex (p : subformula L m₁ (n + 1)) :
+  mlift (∃'p) = ∃'mlift p := by simp[ex_def]
 
-@[simp] lemma zero_arity [has_zero_symbol L] : (0 : term L).arity = 0 :=
-by unfold has_zero.zero; simp
+variables (s : finitary (subterm L m₂ n) m₁)
 
-@[simp] lemma succ_arity [has_succ_symbol L] (t : term L) : (Succ t : term L).arity = t.arity :=
-by unfold has_succ.succ; simp
-
-@[simp] lemma numeral_arity [has_zero_symbol L] [has_succ_symbol L] (n : ℕ) :
-  (n˙ : term L).arity = 0 :=
-by induction n; simp[*, numeral]
-
-@[simp] lemma add_arity [has_add_symbol L] (t u : term L) : (t + u : term L).arity = max t.arity u.arity :=
-by unfold has_add.add; simp
-
-@[simp] lemma mul_arity [has_mul_symbol L] (t u : term L) : (t * u : term L).arity = max t.arity u.arity :=
-by unfold has_mul.mul; simp
-
-@[simp] lemma nested_rew (s₀ s₁) : ∀ (t : term L),
-  (t.rew s₀).rew s₁ = t.rew (λ x, (s₀ x).rew s₁)
-| (#x)       := by simp[rew]
-| (❨f❩ v)  := by simp[rew, nested_rew]
-
-@[simp] lemma rew_id (t : term L) : t.rew ı = t :=
-by induction t; simp[rew]; simp*
-
-lemma rew_rew {s₀ s₁ : ℕ → term L} : ∀ (t : term L),
-  (∀ m, m < t.arity → s₀ m = s₁ m) → t.rew s₀ = t.rew s₁
-| (#x)            h := by simp[rew, arity] at h ⊢; simp*
-| (@app _ n f v)  h := by simp[rew, arity] at h ⊢; refine
-  funext (λ i, rew_rew (v i) (λ m eqn, h m (lt_of_lt_of_le eqn (le_fintype_sup _ i))))
-
-lemma pow_add (t : term L) (i j : ℕ) : (t^i)^j = t^(i + j) :=
-by simp[pow_eq, nested_rew, add_assoc]
-
-@[simp] lemma arity0_rew {t : term L} (h : t.arity = 0) (s : ℕ → term L) : t.rew s = t :=
-by { suffices : rew s t = rew ı t, { simp* },
-     refine rew_rew _ _, simp[h] }
-
-@[simp] lemma arity0_sf {v : term L} (h : v.arity = 0) (i : ℕ) : v^i = v := by simp[has_pow.pow, h]
-
-lemma total_rew_inv
-  (s : ℕ → term L) (h : ∀ n, ∃ m, s m = #n) : ∀ (p : term L) , ∃ q : term L, q.rew s = p
-| (#x) := by rcases h x with ⟨q, h_q⟩; refine ⟨#q, _⟩; simp[h_q]
-| (@app _ n f v) := by rcases classical.skolem.mp (λ i, total_rew_inv (v i)) with ⟨w, w_eqn⟩;
-    refine ⟨❨f❩ w, by simp[w_eqn]⟩
-
-@[simp] lemma pow_0 (t : term L) : t^0 = t := by simp[has_pow.pow]
-
-@[simp] lemma sf_subst_eq (v : term L) (t : term L) (i j : ℕ) (h : j ≤ i) :
-  (v^(i + 1)).rew (ı [j ⇝ t]) = v^i :=
-by { simp[has_pow.pow, rew, nested_rew, h], congr, funext x,
-     have : j < x + (i + 1), from nat.lt_add_left _ _ _ (nat.lt_succ_iff.mpr h),
-     simp[this] }
-
-@[simp] lemma concat_pow_eq (v : term L) (t : term L) (s : ℕ → term L) :
-  (v^1).rew (t ⌢ s) = v.rew s :=
-by simp[concat, rew, pow_eq, nested_rew]
-
-@[simp] lemma rew_arity (t : term L) (s : ℕ → term L) : (t.rew s).arity ≤ ⨆ᶠ (i : fin t.arity), (s i).arity :=
+lemma mlift_rew (p : subformula L m₁ n) : mlift (rew s p) = rew (subterm.mlift ∘ s) p :=
 begin
-  induction t,
-  case var : n { exact le_fintype_sup (λ i : fin (n + 1), (s i).arity) ⟨n, by simp⟩ },
-  case app : n r v IH
-  { simp,refine fintype_sup_le (λ i, _),
-    have : (⨆ᶠ (i : fin (v i).arity), (s i).arity) ≤ (⨆ᶠ (i : fin (❨r❩ v).arity), (s i).arity),
-    { refine fintype_sup_le _, rintros ⟨j, hj⟩,
-      exact le_fintype_sup (λ i : fin (❨r❩ v).arity, (s i).arity) ⟨j, lt_of_lt_of_le hj (le_fintype_sup _ i)⟩ },
-    refine le_trans (IH i) this }
+  induction p; simp[top_eq, equal_eq, imply_eq, neg_eq, fal_eq, subterm.mlift_rew, *],
+  case relation : n p r v { funext x; simp[subterm.mlift_rew] },
+  case fal : n p IH {
+    have : subterm.mlift ∘ subterm.lift ∘ s = subterm.lift ∘ subterm.mlift ∘ s,
+    { funext x; simp[subterm.mlift_lift] },
+    rw[this] }
 end
 
-@[simp] lemma pow_arity (t : term L) (n : ℕ) : (t^n).arity ≤ t.arity + n :=
-begin
-  simp[pow_eq],
-  have lmm₁ : (t.rew (λ x, #(x + n))).arity ≤ (⨆ᶠ (i : fin t.arity), i + n + 1), from rew_arity t (λ x, #(x + n)),
-  have lmm₂ :  (⨆ᶠ (i : fin t.arity), i + n + 1 : ℕ) ≤ (t.arity + n),
-  { refine fintype_sup_le _, rintros ⟨i, hi⟩, simp,
-    from nat.lt_succ_iff.mp (add_lt_add_right (add_lt_add_right hi n) 1) },
-  exact le_trans lmm₁ lmm₂
-end
-
-def vector_vars {n} : vector (term L) n := vector.of_fn $ λ i, #i
-
-@[simp] def symbols : term L → set (Σ n, L.fn n)
-| #n        := ∅ 
-| (app f v) := insert ⟨_, f⟩ (⋃ i, symbols (v i))
-
-lemma symbols_finite : ∀ t : term L, set.finite t.symbols
-| #n        := by simp
-| (app f v) := set.finite.insert ⟨_, f⟩ (set.finite_Union (λ i, symbols_finite (v i)))
-
-inductive subterm : term L → term L → Prop
-| app   : ∀ {n} (f : L.fn n) (v : finitary (term L) n) (i), subterm (v i) (app f v)
-
-@[simp] def complexity : term L → ℕ
-| #n             := 0
-| (@app L n f v) := (⨆ᶠ i, (v i).complexity) + 1
-
-instance : wf_lt (term L) :=
-{ prelt := subterm,
-  wt := complexity,
-  mono' := λ a b h, by { induction h with n f v i, simp,
-  have : (v i).complexity ≤ ⨆ᶠ i, (v i).complexity, from le_fintype_sup (λ i, (v i).complexity) i,
-  exact nat.lt_succ_iff.mpr this } }
-
-@[simp] lemma not_lt_var (t : term L) (n : ℕ) : ¬t < #n := λ h,
-by { rcases wf_lt.lt_iff.mp h with ⟨u, prelt, le⟩, rcases prelt }
-
-@[simp] lemma le_var {t : term L} {n : ℕ} : t ≤ #n ↔ t = #n := by simp[le_iff_lt_or_eq]
-
-@[simp] lemma lt_app {n} (f : L.fn n) (v : fin n → term L) (i) : v i < app f v :=
-by { have : wf_lt.prelt (v i) (app f v), from subterm.app f v i,
-     exact wf_lt.lt_of_prelt this }
-
-@[simp] lemma lt_app_iff {t : term L} {n} {f : L.fn n} {v} : t < app f v ↔ ∃ i, t ≤ v i :=
-⟨by { simp[wf_lt.lt_iff], rintros u prelt le, rcases prelt, refine ⟨_, le⟩ },
- by { rintros ⟨i, le⟩, refine lt_of_le_of_lt le (by simp) }⟩
-
-@[simp] lemma le_app {n} (f : L.fn n) (v : fin n → term L) (i) : v i ≤ app f v :=
-le_of_lt (lt_app f v i)
-
-lemma symbols_ss_of_le {t u : term L} (h : t ≤ u) : t.symbols ⊆ u.symbols :=
-by { induction h,
-  case refl { refl },
-  case of_prelt : a b prelt
-  { induction prelt with n f v i, simp,
-    exact set.subset.trans (show (v i).symbols ⊆ ⋃ i, (v i).symbols, from set.subset_Union _ i) (set.subset_insert _ _) },
-  case trans : s t u _ _ IH_st IH_tu  { exact set.subset.trans IH_st IH_tu } } 
-
-lemma prelt_finite (t : term L) : set.finite {u | subterm u t} :=
-begin
-  induction t,
-  case var 
-  { have : {u : term L | u.subterm #t} = ∅, { ext u, simp, intros h, rcases h },
-    simp[this] },
-  case app : n f v IH
-  { have : {u : term L | u.subterm (❨f❩ v)} = set.range v,
-    { ext u, simp, refine ⟨λ h, _, λ h, _⟩,
-      { rcases h, simp }, { rcases h with ⟨i, rfl⟩, exact subterm.app f v i } },
-    simp[this, set.finite_range] }  
-end
-
-lemma le_finite (t : term L) : set.finite {u | u ≤ t} :=
-wf_lt.le_finite (show ∀ (a : term L), {b : term L | wf_lt.prelt b a}.finite, from prelt_finite) t
-
-@[simp] lemma ite_pow (p : Prop) [decidable p] (t u : term L) (k : ℕ) :
-  (ite p t u)^k = ite p (t^k) (u^k) :=
-by by_cases C : p; simp[C]
-
-lemma rew_inversion_or_le_of_le_rew {t u : term L} {s} (h : t ≤ u.rew s) :
-  (∃ t' ≤ u, t = t'.rew s) ∨ (∃ n, t ≤ s n) :=
-begin
-  induction u,
-  case var : n { simp at h, refine or.inr ⟨n, h⟩ },
-  case app : n f v IH
-  { rcases (eq_or_lt_of_le h) with (rfl | lt),
-    { refine or.inl ⟨app f v, by { refl }, by refl⟩ },
-    { simp at lt, rcases lt with ⟨i, le⟩,
-      rcases IH i le with (⟨t', le', rfl⟩ | ⟨n, le⟩),
-      { refine or.inl ⟨t', (le_trans le' (by simp)), rfl⟩ },
-      { refine or.inr ⟨n, le⟩ } } }
-end
-
-end term
-
-def rewriting_sf_itr (s : ℕ → term L) : ℕ → ℕ → term L
-| 0     := s
-| (n+1) := #0 ⌢ λ x, (rewriting_sf_itr n x)^1
-
-instance : has_pow (ℕ → term L) ℕ := ⟨rewriting_sf_itr⟩
-
-@[simp] lemma rewriting_sf_pow0 (s : ℕ → term L) : (s^0) = s := rfl
-@[simp] lemma rewriting_sf_0 (s : ℕ → term L) (i : ℕ) : (s^(i + 1)) 0 = #0 := rfl
-@[simp] lemma rewriting_sf_1_0 (s : ℕ → term L) (i : ℕ) : (s^1) 0 = #0 := rfl
-@[simp] lemma rewriting_sf_succ (s : ℕ → term L) (n : ℕ) (i : ℕ) : (s^(i + 1)) (n + 1) = (s^i $ n)^1 :=
-by simp[concat, has_pow.pow, rewriting_sf_itr]
-
-lemma rewriting_sf_itr.pow_eq (s : ℕ → term L) (i : ℕ) : (s^(i + 1)) = #0 ⌢ λ x, (s^i $ x)^1 := rfl
+lemma mlift_eq_rew : @mlift L m n = rew (metavar ∘ fin.succ) :=
+by { ext p, induction p; simp[top_eq, equal_eq, imply_eq, neg_eq, fal_eq, subterm.mlift_eq_rew, *],
+     exact eq_rew_of_eq (funext $ λ x, by simp) }
 
-lemma rewriting_sf_itr.pow_add (s : ℕ → term L) (i j : ℕ) : (s^i)^j = s^(i + j) :=
-by { induction j with j IH generalizing s i, { simp },
-     simp[←nat.add_one, ←add_assoc, rewriting_sf_itr.pow_eq, IH] }
-
-@[simp] lemma rewriting_sf_itr_0 (s : ℕ → term L) : s^0 = s := rfl
-
-lemma rewriting_sf_itr_succ (s : ℕ → term L) (n) : s^(n+1) = (s^n)^1 := rfl
-
-lemma rewriting_sf_itr.pow_eq' (s : ℕ → term L) (i : ℕ) :
-  (s^i) = (λ x, if x < i then #x else (s (x - i))^i) :=
-by { induction i with i IH generalizing s, { simp },
-     simp[←nat.add_one, rewriting_sf_itr.pow_eq, IH], funext x,
-     cases x; simp[concat, ←nat.add_one],
-     by_cases C : x < i; simp[C, term.pow_add] }
-
-@[simp] lemma rewriting_sf_itr.pow_app_lt (s : ℕ → term L) {i : ℕ} {x : ℕ} (h : x < i) :
-  (s^i $ x) = #x := by simp[rewriting_sf_itr.pow_eq', h]
-
-@[simp] lemma rewriting_sf_itr.pow_app_ge (s : ℕ → term L) {i : ℕ} {x : ℕ} (h : i ≤ x) :
-  (s^i $ x) = (s (x - i))^i :=
-by {simp[rewriting_sf_itr.pow_eq'], intros lt, exfalso, exact nat.lt_le_antisymm lt h}
-
-@[simp] lemma id_pow (i : ℕ) : (ı : ℕ → term L)^i = ı :=
-by { induction i with i IH, { simp },
-     { simp[rewriting_sf_itr_succ _ i, IH], funext x, cases x; simp } }
-
-lemma id_discard_pow (k i : ℕ) : ((ı-{k})^i : ℕ → term L) = ı-{k + i} :=
-begin
-  funext x,
-  have C : x < i ∨ i ≤ x, from lt_or_ge x i,
-  cases C; simp[C],
-  { have : x < k + i, from nat.lt_add_left x i k C, simp[this] },
-  { have C' : x < k + i ∨ k + i ≤ x, from lt_or_ge x (k + i),
-    cases C'; simp[C'],
-    { have : x - i < k, from (tsub_lt_iff_right C).mpr C',
-      have : x - i + i = x, from nat.sub_add_cancel C,
-      simp* },
-    { have : k ≤ x - i, from (le_tsub_iff_right C).mpr C', simp*, 
-      calc x - i + 1 + i = 1 + (x - i + i) : by simp[add_comm (x - i) 1, add_assoc]
-                     ... = 1 + x : by simp[nat.sub_add_cancel C]
-                     ... = x + 1 : by simp[add_comm 1 x] } }
-end
+@[simp] lemma subst_mlift (u : subterm L m n) (p : subformula L m n) :
+  subst u p.mlift = p :=
+by { simp[mlift_eq_rew, subst, nested_rew], refine rew_eq_self_of_eq (funext $ by simp) _, }
 
-def of_fin {n : ℕ} (v : finitary (term L) n) : ℕ → term L :=
-λ x, if h : x < n then v ⟨x, h⟩ else #(x - n)
-
-@[simp] lemma of_fin_app_of_lt {n : ℕ} (v : finitary (term L) n) {x : ℕ} (lt : x < n) :
-  of_fin v x = v ⟨x, lt⟩ :=
-by simp[of_fin, lt]
-
-@[simp] lemma of_fin_app_of_le {n : ℕ} (v : finitary (term L) n) {x : ℕ} (le : n ≤ x) :
-  of_fin v x = #(x - n) :=
-by simp[of_fin, le]
-
-@[simp] lemma of_fin_0 (t : term L) : of_fin‹t› 0 = t := by simp
-
-@[simp] lemma of_fin_eq_nil (v : finitary (term L) 0) : of_fin v = ı :=
-by funext x; simp
-
-@[simp] lemma of_fin_of_lt {n} (v : finitary (term L) n) (m : ℕ) {x} (lt : x < m) : (of_fin v^m) x = #x :=
-by simp[rewriting_sf_itr.pow_eq', lt]
-
-@[simp] lemma of_fin_of_ge {n} (v : finitary (term L) n) (m : ℕ) {x} (ge : m + n ≤ x) : (of_fin v^m) x = #(x - n) :=
-by { simp[rewriting_sf_itr.pow_eq', ge, show ¬x < m, by omega, show n ≤ x - m, by omega], omega }
+lemma mlift_subst (u : subterm L m n) (p : subformula L (m + 1) n) :
+  mlift (subst u p) = rew (@fin.cases m (λ _, subterm L (m + 1) n) u.mlift (subterm.mlift ∘ metavar)) p :=
+by simp[subst, mlift_rew]; refine eq_rew_of_eq (funext $ λ x, by rcases (fin.eq_zero_or_eq_succ x) with (rfl | ⟨x, rfl⟩); simp)
 
-@[simp] lemma of_fin_of_eq (t : term L) (m : ℕ) : (of_fin ‹t›^m) m = t^m := by simp
-
-@[simp] lemma of_fin_of_gt (t : term L) (m : ℕ) {x} (ge : m < x) : (of_fin ‹t›^m) x = #(x - 1) :=
-of_fin_of_ge ‹t› m (nat.succ_le_iff.mpr ge)
-
-lemma rewriting_sf_perm {s : ℕ → term L} (h : ∀ n, ∃ m, s m = #n) : ∀ n, ∃ m, (s^1) m = #n :=
-λ n, by { cases n, refine ⟨0, by simp⟩,
-          rcases h n with ⟨m, e_m⟩, refine ⟨m+1, _⟩, simp[e_m] }
-
-@[simp] def formula.arity : formula L → ℕ
-| ⊤                 := 0
-| (formula.app p v) := ⨆ᶠ i, (v i).arity
-| (t ≃ u)          := max t.arity u.arity
-| (p ⟶ q)           := max p.arity q.arity
-| (∼p)              := p.arity
-| (∀.p)             := p.arity - 1
-
-@[reducible] def formula.is_sentence : formula L → Prop := λ p, p.arity = 0
-
-@[simp] lemma formula.and_arity (p q : formula L) : (p ⊓ q).arity = max p.arity q.arity :=
-by simp[has_inf.inf, formula.and]
-
-@[simp] lemma formula.or_arity (p q : formula L) : (p ⊔ q).arity = max p.arity q.arity :=
-by simp[has_sup.sup, formula.or]
-
-@[simp] lemma formula.iff_arity (p q : formula L) : (p ⟷ q).arity = max p.arity q.arity :=
-by simp[lrarrow_def]; exact max_comm _ _
-
-@[simp] lemma formula.bot_arity : (⊥ : formula L).arity = 0 :=
-by simp[has_bot.bot]
+end mlift
 
-@[simp] lemma formula.ex_arity (p : formula L) : (∃. p : formula L).arity = p.arity - 1 :=
-by simp[has_exists_quantifier.ex, formula.ex]
+def push' {m} : Π {n}, subformula L m (n + 1) → subformula L (m + 1) n
+| n verum          := ⊤
+| n (relation p v) := relation p (subterm.push ∘ v)
+| n (equal t u)    := t.push =' u.push
+| n (imply p q)    := p.push' ⟶ q.push'
+| n (neg p)        := ∼p.push'
+| n (fal p)        := ∀'p.push'
+using_well_founded {rel_tac := λ _ _, `[exact ⟨_, measure_wf (λ x, x.2.complexity)⟩]}
 
-lemma subst_pow (t : term L) (n i : ℕ) : ı[n ⇝ t]^i = ı[n + i ⇝ t^i] :=
-begin
-  induction i with i IH, { simp }, funext x,
-  cases x; simp[←nat.add_one, ←add_assoc, IH],
-  { have T : x < n + i ∨ x = n + i ∨ n + i < x, exact trichotomous _ _,
-    cases T, { simp[T], }, cases T; simp[T, pow_add, term.pow_add],
-    { have : 0 < x, exact pos_of_gt T, exact (nat.pos_succ this).symm} }
-end
+def push : subformula L m (n + 1) →ₗ subformula L (m + 1) n :=
+{ to_fun := push',
+  map_neg' := λ p, by unfold has_negation.neg; simp[push']; refl,
+  map_imply' := λ p q, by unfold has_arrow.arrow; simp[push']; refl,
+  map_and' := λ p q, by unfold has_inf.inf; simp[and, push']; refl,
+  map_or' := λ p q, by unfold has_sup.sup; simp[or, push']; refl,
+  map_top' := by unfold has_top.top; simp[push']; refl,
+  map_bot' := by unfold has_bot.bot; simp[push']; refl }
 
-lemma term.pow_rew_distrib (t : term L) (s : ℕ → term L) (i : ℕ): (t.rew s)^i = (t^i).rew (s^i) :=
-by { induction i with i IH generalizong s i, { simp, },
-     { simp[←nat.add_one, term.pow_add, rewriting_sf_itr.pow_add, rewriting_sf_itr.pow_eq',
-         IH, term.pow_eq, term.nested_rew] } }
+section push
 
-@[simp] lemma rew_subst_id : (λ x, (((λ x, #(x + 1)) ^ 1) x).rew ı[0 ⇝ #0]  : ℕ → term L) = ı :=
-by { funext x, cases x; simp }
+lemma push_def (p : subformula L m (n + 1)) : push p = push' p := rfl
 
-@[simp] lemma rew_slide_eq_concat (s : ℕ → term L) (t : term L) :
-  (λ x, ((s^1) x).rew ı[0 ⇝ t]) = t ⌢ s :=
-funext (λ y, by cases y; simp)
+@[simp] lemma push_relation {p} (r : L.pr p) (v : finitary (subterm L m (n + 1)) p) :
+  push (relation r v) = relation r (subterm.push ∘ v) := by simp[push_def, push']
 
-@[simp] lemma concat_eq_id :
-  (#0 ⌢ (λ x, #(x + 1)) : ℕ → term L) = ı :=
-funext (λ x, by cases x; simp)
+@[simp] lemma push_equal (t u : subterm L m (n + 1)) :
+  push (t =' u : subformula L m (n + 1)) = (t.push =' u.push) := by unfold has_eq.eq; simp[push_def, push']; refl
 
-namespace formula
-
-@[simp] lemma constant_arity (c : L.pr 0) {v : finitary (term L) 0} : (❴c❵ v).arity = 0 :=
-by simp
-
-@[simp] lemma unary_arity (p : L.pr 1) (v : finitary (term L) 1) : (❴p❵ v).arity = (v 0).arity :=
-by simp
-
-@[simp] lemma binary_arity (p : L.pr 2) (v : finitary (term L) 2) :
-  (❴p❵ v).arity = max (v 0).arity (v 1).arity :=
-by simp; exact max_comm _ _
+@[simp] lemma push_fal (p : subformula L m (n + 1 + 1)) :
+  push (∀'p) = ∀'push p := by unfold has_univ_quantifier'.univ; simp[push_def, push']; refl
 
-@[simp] lemma le_arity [has_le_symbol L] (t u : term L) : (t ≼ u : formula L).arity = max t.arity u.arity :=
-by unfold has_preceq.preceq; simp
+@[simp] lemma push_ex (p : subformula L m₁ (n + 1 + 1)) :
+  push (∃'p) = ∃'push p := by simp[ex_def]
 
-@[simp] lemma mem_arity [has_mem_symbol L] (t u : term L) : (t ∊ u : formula L).arity = max t.arity u.arity :=
-by unfold has_elem.elem; simp
-
-@[simp] def rew : (ℕ → term L) → formula L → formula L
-| s ⊤         := ⊤
-| s (app p v) := app p (λ i, (v i).rew s)
-| s (t ≃ u)  := (t.rew s) ≃ (u.rew s)
-| s (p ⟶ q)  := p.rew s ⟶ q.rew s
-| s (∼p)      := ∼(p.rew s)
-| s (∀.p)   := ∀.(p.rew (s^1))
-
-@[reducible] def rew_var (s : ℕ → ℕ) : formula L → formula L := λ p, p.rew (λ x, #(s x))
-
-@[simp] lemma constant_rew (p : L.pr 0) (s : ℕ → term L) {v : finitary (term L) 0} :
-  (❴p❵ v).rew s = ❴p❵ finitary.nil :=
-by simp
-
-@[simp] lemma unary_rew (p : L.pr 1) (s : ℕ → term L) (v : finitary (term L) 1) : (❴p❵ v).rew s = ❴p❵ ‹(v 0).rew s› :=
-by simp; ext; simp
-
-@[simp] lemma binary_rew (p : L.pr 2) (s : ℕ → term L) (v : finitary (term L) 2) :
-  (❴p❵ v).rew s = ❴p❵ ‹(v 0).rew s, (v 1).rew s› :=
-by simp; ext; simp
-
-@[simp] lemma le_rew [has_le_symbol L] (t u : term L) (s : ℕ → term L) :
-  (t ≼ u : formula L).rew s = (t.rew s ≼ u.rew s) :=
-by unfold has_preceq.preceq; simp
-
-@[simp] lemma mem_rew [has_mem_symbol L] (t u : term L) (s : ℕ → term L) :
-  (t ∊ u : formula L).rew s = (t.rew s ∊ u.rew s) :=
-by unfold has_elem.elem; simp
-
-@[simp] lemma and_rew (p q : formula L) (s) : (p ⊓ q).rew s = p.rew s ⊓ q.rew s := by simp[has_inf.inf, and, formula.rew]
-@[simp] lemma or_rew (p q : formula L) (s) : (p ⊔ q).rew s = p.rew s ⊔ q.rew s := by simp[has_sup.sup, or, formula.rew]
-@[simp] lemma iff_rew (p q : formula L) (s) : (p ⟷ q).rew s = p.rew s ⟷ q.rew s := by simp[lrarrow_def, formula.rew]
-@[simp] lemma nfal_rew (p : formula L) (i : ℕ) (s) : (nfal p i).rew s = nfal (p.rew (s^i)) i :=
-by { induction i with i IH generalizing s, { simp },
-     simp[←nat.add_one, IH, rewriting_sf_itr.pow_add, add_comm 1 i] }
-@[simp] lemma ex_rew (p : formula L) (s) : (∃. p).rew s = ∃. p.rew (s^1) :=by simp[has_exists_quantifier.ex, ex]
-@[simp] lemma bot_rew (s) : (⊥ : formula L).rew s = ⊥ := by simp[has_bot.bot]
-
-@[simp] lemma rew_id (p : formula L) : p.rew ı = p :=
-by { induction p; try { simp[rew] }; try {simp*} }
-
-@[simp] lemma inf_conjunction_rew {n} (P : finitary (formula L) n) (s) :
-  (inf_conjunction n P).rew s = ⋀ i, (P i).rew s :=
-by { induction n with n IH; simp* }
-
-@[simp] lemma sup_disjunction_rew {n} (P : finitary (formula L) n) (s) :
-  (sup_disjunction n P).rew s = ⋁ i, (P i).rew s :=
-by { induction n with n IH; simp* }
-
-instance : has_pow (formula L) ℕ := ⟨λ p i, p.rew (λ x, #(x + i))⟩
-
-lemma pow_eq (p : formula L) (i : ℕ) : p^i = p.rew (λ x, #(x + i)) := rfl
-
-@[simp] lemma formula_pow_0 (p : formula L) : p^0 = p := by simp[has_pow.pow]
-
-@[simp] lemma app_pow {n} (p : L.pr n) (v : finitary (term L) n) (i : ℕ) : (❴p❵ v)^i = ❴p❵ (v^i) := rfl
-
-@[simp] lemma constant_pow (c : L.pr 0) (i : ℕ) {v : finitary (term L) 0} : (app c v)^i = app c finitary.nil :=
-by simp
-
-@[simp] lemma unary_pow (p : L.pr 1) (i : ℕ) (t : term L) : (❴p❵ ‹t›)^i = ❴p❵ ‹t^i› :=
-by simp[pow_eq]; refl
-
-@[simp] lemma binary_pow (p : L.pr 2) (i : ℕ) (t₁ t₂ : term L) :
-  (❴p❵ ‹t₁, t₂›)^i = ❴p❵ ‹t₁^i, t₂^i› :=
-by simp[pow_eq]; refl
-
-@[simp] lemma le_pow [has_le_symbol L] (t u : term L) (i : ℕ) :
-  (t ≼ u : formula L)^i = (t^i ≼ u^i) :=
-by simp[pow_eq]; refl
-
-@[simp] lemma mem_pow [has_mem_symbol L] (t u : term L) (i : ℕ) :
-  (t ∊ u : formula L)^i = (t^i ∊ u^i) :=
-by simp[pow_eq]; refl
-
-@[simp] lemma top_pow (i : ℕ) : (⊤ : formula L)^i = ⊤ := by refl
-@[simp] lemma bot_pow (i : ℕ) : (⊥ : formula L)^i = ⊥ := by refl
-@[simp] lemma eq_pow (t u : term L) (i : ℕ) : (t ≃ u : formula L)^i = (t^i ≃ u^i) := rfl
-@[simp] lemma imply_pow (p q : formula L) (i : ℕ) : (p ⟶ q)^i = p^i ⟶ q^i := rfl
-@[simp] lemma neg_pow (p : formula L) (i : ℕ) : (∼p)^i = ∼(p^i) := rfl
-@[simp] lemma and_pow (p q : formula L) (i : ℕ) : (p ⊓ q)^i = (p^i) ⊓ (q^i) := rfl
-@[simp] lemma inf_conjunction_pow {n} (P : finitary (formula L) n) (i : ℕ) : (inf_conjunction n P)^i = ⋀ j, (P j)^i :=
-by induction n with n IH; simp*
-@[simp] lemma or_pow (p q : formula L) (i : ℕ) : (p ⊔ q)^i = (p^i) ⊔ (q^i) := rfl
-@[simp] lemma sup_disjunction_pow {n} (P : finitary (formula L) n) (i : ℕ) : (sup_disjunction n P)^i = ⋁ j, (P j)^i :=
-by induction n with n IH; simp*
-
-lemma fal_pow (p : formula L) (i : ℕ) : (∀.p)^i = ∀.p.rew (#0 ⌢ λ x, #(x + i + 1)) :=
-by simp[formula.pow_eq, rewriting_sf_itr.pow_eq]
-
-lemma fal_pow_discard (p : formula L) : (∀.p)^1 = ∀.p.rew ı-{1} :=
-by { simp[formula.pow_eq, rewriting_sf_itr.pow_eq, discard], congr, funext x, cases x; simp }
-
-lemma ex_pow_discard (p : formula L) : (∃. p)^1 = ∃. p.rew ı-{1} :=
-by { simp[formula.pow_eq, rewriting_sf_itr.pow_eq, discard], congr, funext x, cases x; simp }
-
-lemma nfal_pow (p : formula L) (n i : ℕ) :
-  (nfal p n)^i = nfal (p.rew (λ x, if x < n then #x else #(x + i))) n :=
-by { simp[formula.pow_eq, rewriting_sf_itr.pow_eq'], congr, funext x,
-     by_cases C : x < n; simp[C], omega }
-
-lemma nested_rew : ∀ (p : formula L) (s₀ s₁),
-  (p.rew s₀).rew s₁ = p.rew (λ x, (s₀ x).rew s₁)
-| ⊤         _ _ := by simp
-| (❴p❵ v) _ _ := by simp[rew]
-| (t ≃ u)  _ _ := by simp[rew]
-| (p ⟶ q)   _ _ := by simp[rew, nested_rew p, nested_rew q]
-| (∼p)      _ _ := by simp[rew]; refine nested_rew p _ _
-| (∀.p)     _ _ := by { simp[rew, nested_rew p], congr,
-    funext n, cases n; simp, simp[concat, rewriting_sf_itr.pow_eq, term.pow_eq] }
-
-lemma rew_rew : ∀ (p : formula L) {s₀ s₁ : ℕ → term L},
-  (∀ m, m < p.arity → s₀ m = s₁ m) → p.rew s₀ = p.rew s₁
-| ⊤         _ _ _ := by simp
-| (❴p❵ v) _ _ h := by simp[rew, arity] at h ⊢; refine funext
-    (λ i, term.rew_rew (v i) (λ m eqn, h _ $ lt_of_lt_of_le eqn (le_fintype_sup _ i)))
-| (t ≃ u)  _ _ h := by simp[rew, arity] at h ⊢;
-    { refine ⟨term.rew_rew _ (λ _ e, h _ (or.inl e)), term.rew_rew _ (λ _ e, h _ (or.inr e))⟩ }
-| (p ⟶ q)   _ _ h := by simp[rew, arity] at h ⊢;
-    refine ⟨rew_rew _ (λ _ e, h _ (or.inl e)), rew_rew _ (λ _ e, h _ (or.inr e))⟩
-| (∼p)      _ _ h := by simp[rew, arity] at h ⊢; refine rew_rew _ h
-| (∀.p)     _ _ h := by { simp[rew, arity] at h ⊢,
-    refine rew_rew _ (λ m e, _), cases m; simp,
-    cases p.arity, { exfalso, simp* at* },
-    { simp at h, simp[h _ (nat.succ_lt_succ_iff.mp e)] } }
-
-lemma pow_add (p : formula L) (i j : ℕ) : (p^i)^j = p^(i + j) :=
-by simp[pow_eq, nested_rew, add_assoc]
-
-@[simp] lemma is_sentence_rew {p : formula L} (h : is_sentence p) (s : ℕ → term L) : p.rew s = p :=
-by { suffices : rew s p = rew ı p, { simp* },
-     refine rew_rew _ _, simp[show p.arity = 0, from h] }
-
-@[simp] lemma is_sentence_sf {p : formula L} (h : is_sentence p) (i : ℕ) : p^i = p :=
-by simp[has_pow.pow, is_sentence_rew h]
-
-@[simp] lemma sf_subst_eq (p : formula L) (t : term L) (i j : ℕ) (h : j ≤ i) : (p^(i + 1)).rew ı[j ⇝ t] = p^i :=
-by { simp[has_pow.pow, nested_rew, h], congr, funext x,
-     have : j < x + (i + 1), from nat.lt_add_left _ _ _ (nat.lt_succ_iff.mpr h),
-     simp[this] }
-
-lemma subst_sf_rew (p : formula L) (t : term L) (s : ℕ → term L) :
-  (p.rew ı[0 ⇝ t]).rew s = (p.rew (s^1)).rew ı[0 ⇝ t.rew s] :=
-by { simp[formula.rew, nested_rew], congr, ext n, cases n; simp }
-
-@[simp] lemma sf_subst_eq_0 (p : formula L) (t) : (p^1).rew ı[0 ⇝ t] = p :=
-by simp[nested_rew]
-
-lemma pow_rew_distrib  (p : formula L) (s : ℕ → term L) (i : ℕ): (p.rew s)^i = (p^i).rew (s^i) :=
-by { induction i with i IH generalizong s i, { simp },
-     { simp[←nat.add_one, ←pow_add, ←rewriting_sf_itr.pow_add, IH, formula.pow_eq _ 1, nested_rew], refl } }
-
-lemma total_rew_inv :
-  ∀ (s : ℕ → term L) (h : ∀ n, ∃ m, s m = #n) (p : formula L), ∃ q : formula L, q.rew s = p
-| _ _ ⊤              := ⟨⊤, by simp⟩
-| s h (@app _ n p v) := by rcases classical.skolem.mp (λ i : fin n, @term.total_rew_inv _ s h (v i : term L)) with ⟨w, w_p⟩;
-    refine ⟨❴p❵ w, by simp[w_p]⟩
-| s h (t ≃ u)       := 
-    by rcases term.total_rew_inv s h t with ⟨w₁, e_w₁⟩;
-       rcases term.total_rew_inv s h u with ⟨w₂, e_w₂⟩; refine ⟨w₁ ≃ w₂, by simp[e_w₁, e_w₂]⟩
-| s h (p ⟶ q)        := 
-    by rcases total_rew_inv s h p with ⟨p', e_p'⟩;
-       rcases total_rew_inv s h q with ⟨q', e_q'⟩; refine ⟨p' ⟶ q', by simp*⟩
-| s h (∼p)           := by rcases total_rew_inv s h p with ⟨q, e_q⟩; refine ⟨∼q, by simp*⟩
-| s h (∀.p)          := by rcases total_rew_inv _ (rewriting_sf_perm h) p with ⟨q, e_q⟩; refine ⟨∀.q, by simp[e_q]⟩
-
-@[simp] lemma rew_var_inj_of_inj :
-  ∀ {p q : formula L} {s : ℕ → ℕ} (I : function.injective s),
-  p.rew_var s = q.rew_var s ↔ p = q
-| ⊤                   p                   s I := by {cases p; simp[rew_var], }
-| (formula.app p v)   ⊤                   s I := by simp[rew_var]
-| (formula.app p₁ v₁) (formula.app p₂ v₂) s I := by { simp[rew_var], rintros rfl rfl,
-    simp, split,
-    { intros h, funext i,
-      have : term.rew_var s (v₁ i) = term.rew_var s (v₂ i), from congr_fun h i,
-      exact (term.rew_var_inj_of_inj I).mp this },
-    { rintros rfl, simp } }
-| (formula.app p v)   (t ≃ u)            s I := by simp[rew_var]
-| (formula.app r v)   (p ⟶ q)             s I := by simp[rew_var]
-| (formula.app r v)   (∼p)                s I := by simp[rew_var]
-| (formula.app r v)   (∀.p)               s I := by simp[rew_var, fal_pow]
-| (t ≃ u)            p                   s I := by cases p; simp[rew_var, fal_pow, I]
-| (p ⟶ q)             r                   s I :=
-    by cases r; simp[rew_var, fal_pow, @rew_var_inj_of_inj p _ s I, @rew_var_inj_of_inj q _ s I]
-| (∼p)                q                   s I :=
-    by cases q; simp[rew_var, fal_pow, @rew_var_inj_of_inj p _ s I]
-| (∀.p)               ⊤                   s I := by simp[rew_var]
-| (∀.p)               (formula.app r v)   s I := by simp[rew_var]
-| (∀.p)               (t ≃ u)            s I := by simp[rew_var]
-| (∀.p)               (q ⟶ r)             s I := by simp[rew_var]
-| (∀.p)               (∼q)                s I := by simp[rew_var]
-| (∀.p)               (∀.q)               s I := by {simp[rew_var, fal_pow], 
-    have : ∀ p : formula L, p.rew ((λ x, #(s x))^1) = p.rew_var (λ x, if x = 0 then 0 else s (x - 1) + 1),
-    { intros p, simp[rewriting_sf_itr.pow_eq', rew_var, nested_rew], congr, funext x, cases x; simp },
-    
-    have I' : function.injective (λ x, if x = 0 then 0 else s (x - 1) + 1),
-    { intros x y, cases x; cases y; simp,
-      { intros h, exfalso, exact (nat.succ_ne_zero _).symm h }, { exact (@I x y) } },
-    simp[this, @rew_var_inj_of_inj p q _ I'] }
-  
-@[simp] lemma pow_inj : ∀ {p q : formula L} {i : ℕ}, p^i = q^i ↔ p = q :=
-λ p q i, by { simp[has_pow.pow], refine rew_var_inj_of_inj (λ x y, by simp) }
-
-@[simp] def is_open : Theory L
-| ⊤          := true
-| (❴p❵ v)  := true
-| (t ≃ u)   := true
-| (p ⟶ q)    := p.is_open ∧ q.is_open
-| (∼p)       := p.is_open
-| (∀.p)      := false
-
-@[simp] lemma is_open.and (p q : formula L) : (p ⊓ q).is_open ↔ p.is_open ∧ q.is_open := by refl
-
-@[simp] lemma is_open.or (p q : formula L) : (p ⊔ q).is_open ↔ p.is_open ∧ q.is_open := by refl
-
-@[simp] lemma is_open.bot : (⊥ : formula L).is_open := by simp[has_bot.bot]
-
-@[simp] lemma is_open.ex (p : formula L) : ¬(∃. p).is_open := by simp[formula.ex_eq]
-
-@[simp] def is_open_rew : ∀ {p : formula L} {s}, (p.rew s).is_open ↔ p.is_open
-| ⊤        s := by simp
-| (❴p❵ v)  s := by simp
-| (t ≃ u) s := by simp
-| (p ⟶ q) s  := by simp[@is_open_rew p s, @is_open_rew q s]
-| (∼p)     s := by simp[@is_open_rew p s]
-| (∀.p)  s   := by simp
-
-@[simp] def is_open_pow : ∀ {p : formula L} {i : ℕ}, (p^i).is_open ↔ p.is_open :=
-by simp[pow_eq]
-
-@[simp] lemma is_open.le [has_le_symbol L] (t u : term L) : (t ≼ u : formula L).is_open := by simp[has_preceq.preceq]
-
-@[simp] lemma is_open.mem [has_mem_symbol L] (t u : term L) : (t ∊ u : formula L).is_open := by simp[has_elem.elem]
-
-@[simp] lemma nfal_arity : ∀ (n) (p : formula L), (nfal p n).arity = p.arity - n
-| 0     p := by simp[formula.arity]
-| (n+1) p := by {simp[formula.arity, nfal_arity n], exact (arity p).sub_sub _ _ }
-
-lemma nfal_is_sentence (p : formula L) : is_sentence (nfal p p.arity) :=
-by simp[is_sentence]
-
-@[simp] lemma conjunction_arity {n} {v : finitary (formula L) n} :
-  (inf_conjunction n v).arity = ⨆ᶠ i, (v i).arity :=
-by { induction n with n IH; simp*,
-  refine le_antisymm _ _; simp,
-  { split,
-    { refine le_fintype_sup' ⟨n, by simp[←nat.add_one]⟩ (by refl) },
-    { refine fintype_sup_le _, rintros ⟨i, hi⟩, refine le_fintype_sup' ⟨i, by omega⟩ (by refl) } },
-  { have : (v ⟨n, by simp[←nat.add_one]⟩).arity ≤  (⨆ᶠ (i : fin n), (v ⟨i, by simp[←nat.add_one]⟩).arity) ∨
-           (⨆ᶠ (i : fin n), (v ⟨i, by simp[←nat.add_one]⟩).arity) ≤ (v ⟨n, by simp[←nat.add_one]⟩).arity,
-      from le_total _ _, rcases this with (le | le),
-    { refine or.inr (fintype_sup_le _), rintros ⟨i, hi⟩,
-      have : i = n ∨ i < n, from eq_or_lt_of_le (nat.lt_succ_iff.mp hi), rcases this with (rfl | lt),
-      { simpa using le }, { refine le_fintype_sup' ⟨i, lt⟩ (by refl) } },
-    { refine or.inl (fintype_sup_le _), rintros ⟨i, hi⟩,
-      have : i = n ∨ i < n, from eq_or_lt_of_le (nat.lt_succ_iff.mp hi), rcases this with (rfl | lt),
-      { refl }, { refine le_trans _ le, refine le_fintype_sup' ⟨i, lt⟩ (by refl) } } } }
-
-@[simp] lemma disjunction_arity {n} {v : finitary (formula L) n} :
-  (sup_disjunction n v).arity = ⨆ᶠ i, (v i).arity :=
-by { induction n with n IH; simp*,
-  refine le_antisymm _ _; simp,
-  { split,
-    { refine le_fintype_sup' ⟨n, by simp[←nat.add_one]⟩ (by refl) },
-    { refine fintype_sup_le _, rintros ⟨i, hi⟩, refine le_fintype_sup' ⟨i, by omega⟩ (by refl) } },
-  { have : (v ⟨n, by simp[←nat.add_one]⟩).arity ≤  (⨆ᶠ (i : fin n), (v ⟨i, by simp[←nat.add_one]⟩).arity) ∨
-           (⨆ᶠ (i : fin n), (v ⟨i, by simp[←nat.add_one]⟩).arity) ≤ (v ⟨n, by simp[←nat.add_one]⟩).arity,
-      from le_total _ _, rcases this with (le | le),
-    { refine or.inr (fintype_sup_le _), rintros ⟨i, hi⟩,
-      have : i = n ∨ i < n, from eq_or_lt_of_le (nat.lt_succ_iff.mp hi), rcases this with (rfl | lt),
-      { simpa using le }, { refine le_fintype_sup' ⟨i, lt⟩ (by refl) } },
-    { refine or.inl (fintype_sup_le _), rintros ⟨i, hi⟩,
-      have : i = n ∨ i < n, from eq_or_lt_of_le (nat.lt_succ_iff.mp hi), rcases this with (rfl | lt),
-      { refl }, { refine le_trans _ le, refine le_fintype_sup' ⟨i, lt⟩ (by refl) } } } }
-
-def fal_complete (p : formula L) := ∀.[p.arity] p
-
-prefix `∀.* `:64 := fal_complete
-
-@[simp] lemma fal_complete_is_sentence (p : formula L) : is_sentence (∀.* p) :=
-by simp[is_sentence, fal_complete]
-
-@[simp] lemma is_sentence_verum_iff : is_sentence (⊤ : formula L) := by simp[is_sentence]
-
-@[simp] lemma is_sentence_app_iff {n} (r : L.pr n) (v) : is_sentence (app r v) ↔ ∀ i, (v i).arity = 0 :=
-by {simp[is_sentence], sorry }
-
-@[simp] lemma is_sentence_neg_iff {p : formula L} : is_sentence (∼p) ↔ is_sentence p := by simp[is_sentence]
-
-@[simp] lemma is_sentence_imply_iff {p q: formula L} : is_sentence (p ⟶ q) ↔ is_sentence p ∧ is_sentence q := by simp[is_sentence]
-
-@[simp] lemma is_sentence_and_iff {p q: formula L} : is_sentence (p ⊓ q) ↔ is_sentence p ∧ is_sentence q := by simp[is_sentence]
-
-@[simp] lemma is_sentence_or_iff {p q: formula L} : is_sentence (p ⊔ q) ↔ is_sentence p ∧ is_sentence q := by simp[is_sentence]
-
-@[simp] lemma is_sentence_fal_iff {p : formula L} : is_sentence (∀.p) ↔ p.arity ≤ 1 := by simp[is_sentence]
-
-@[simp] lemma is_sentence_ex_iff {p : formula L} : is_sentence (∃. p) ↔ p.arity ≤ 1 := by simp[is_sentence]
-
-lemma rew_arity (p : formula L) (s : ℕ → term L) : (p.rew s).arity ≤ ⨆ᶠ (i : fin p.arity), (s i).arity :=
-begin
-  induction p generalizing s,
-  case app : n r v
-  { simp, refine fintype_sup_le (λ i, _),
-    have : (⨆ᶠ (j : fin (v i).arity), (s j).arity) ≤ (⨆ᶠ (i : fin (❴r❵ v).arity), (s i).arity),
-    { refine fintype_sup_le _, rintros ⟨j, hj⟩, simp,
-      refine le_fintype_sup' ⟨j, lt_of_lt_of_le hj (by simp; exact le_fintype_sup' i (by simp))⟩ (by simp) },
-    exact le_trans ((v i).rew_arity s) this },
-  case equal : t u
-  { simp, refine ⟨le_trans (t.rew_arity s) (fintype_sup_le _), le_trans (u.rew_arity s) (fintype_sup_le _)⟩,
-    { rintros ⟨i, hi⟩, refine le_fintype_sup' ⟨i, by simp[hi]⟩ (by simp) },
-    { rintros ⟨i, hi⟩, refine le_fintype_sup' ⟨i, by simp[hi]⟩ (by simp) } },
-  case verum { simp },
-  case imply : p q IH_p IH_q
-  { simp, refine ⟨le_trans (IH_p s) (fintype_sup_le _), le_trans (IH_q s) (fintype_sup_le _)⟩,
-    { rintros ⟨i, hi⟩, refine le_fintype_sup' ⟨i, by simp[hi]⟩ (by simp) },
-    { rintros ⟨i, hi⟩, refine le_fintype_sup' ⟨i, by simp[hi]⟩ (by simp) } },
-  case neg : p IH
-  { simp, refine le_trans (IH s) (fintype_sup_le _),
-    rintros ⟨i, hi⟩, refine le_fintype_sup' ⟨i, by simp[hi]⟩ (by simp) },
-  case fal : p IH
-  { have : (⨆ᶠ (i : fin p.arity), ((s ^ 1) i).arity) ≤ ((⨆ᶠ  (i : fin (∀.p).arity), (s i).arity) + 1),
-    { refine fintype_sup_le _, rintros ⟨i, hi⟩,
-      cases i; simp,
-      have : (s i).arity ≤ (⨆ᶠ (i : fin (∀.p).arity), (s i).arity), from le_fintype_sup (λ (i : fin (∀.p).arity), (s i).arity) ⟨i, by simp; omega⟩,
-      refine le_trans (show (s i ^ 1).arity ≤ (s i).arity + 1, by simp) (by simp[this]) },
-    simp, exact le_trans (IH (s^1)) this }
-end
-
-@[simp] lemma pow_arity (p : formula L) (n : ℕ) : (p^n).arity ≤ p.arity + n :=
-begin
-  simp[pow_eq],
-  have lmm₁ : (p.rew (λ x, #(x + n))).arity ≤ (⨆ᶠ (i : fin p.arity), i + n + 1), from p.rew_arity (λ x, #(x + n)),
-  have lmm₂ :  (⨆ᶠ (i : fin p.arity), i + n + 1 : ℕ) ≤ (p.arity + n),
-  { refine fintype_sup_le _, rintros ⟨i, hi⟩, simp,
-    from nat.lt_succ_iff.mp (add_lt_add_right (add_lt_add_right hi n) 1) },
-  exact le_trans lmm₁ lmm₂
-end
-
-@[simp] lemma subst_arity (p : formula L) (n : ℕ) (t : term L) :
-  (p.rew ı[n ⇝ t]).arity ≤ max t.arity (p.arity + 1) :=
-begin
-  have : (⨆ᶠ (i : fin p.arity), (ı[n ⇝ t] i).arity) ≤ max t.arity (p.arity + 1),
-  { refine fintype_sup_le _, rintros ⟨i, hi⟩, simp,
-    have : i < n ∨ i = n ∨ n < i, from trichotomous i n, rcases this with (lt | rfl | lt); simp*,
-    { simp[le_of_lt hi] }, { simp[show i ≤ p.arity + 1, from le_add_right (le_of_lt hi)] } },
-  exact le_trans (p.rew_arity ı[n ⇝ t]) this
-end
-
-@[simp] def fn_symbols : formula L → set (Σ n, L.fn n)
-| ⊤         := ∅
-| (app r v) := ⋃ i, (v i).symbols
-| (t ≃ u)  := t.symbols ∪ u.symbols
-| (p ⟶ q)   := fn_symbols p ∪ q.fn_symbols
-| (∼p)      := p.fn_symbols
-| (∀.p)     := p.fn_symbols
-
-def fn_symbols' (p : formula L) (n : ℕ) : set (L.fn n) := {f | (⟨n, f⟩ : Σ n, L.fn n) ∈ p.fn_symbols }
-
-lemma mem_fn_symbols'_iff {n : ℕ} {f : L.fn n} {p : formula L} :
-  f ∈ p.fn_symbols' n ↔ (⟨n, f⟩ : Σ n, L.fn n) ∈ p.fn_symbols :=
-by simp[fn_symbols']
-
-@[simp] def pr_symbols : formula L → set (Σ n, L.pr n)
-| ⊤         := ∅
-| (app r v) := {⟨_, r⟩}
-| (t ≃ u)  := ∅
-| (p ⟶ q)   := p.pr_symbols ∪ q.pr_symbols
-| (∼p)      := p.pr_symbols
-| (∀.p)     := p.pr_symbols
-
-def pr_symbols' (p : formula L) (n : ℕ) : set (L.pr n) := {r | (⟨n, r⟩ : Σ n, L.pr n) ∈ p.pr_symbols }
-
-lemma mem_pr_symbols'_iff {n : ℕ} {r : L.pr n} {p : formula L} :
-  r ∈ p.pr_symbols' n ↔ (⟨n, r⟩ : Σ n, L.pr n) ∈ p.pr_symbols :=
-by simp[pr_symbols']
-
-lemma fn_symbols_finite : ∀ p : formula L, p.fn_symbols.finite
-| ⊤         := by simp
-| (app r v) := set.finite_Union (λ i, (v i).symbols_finite)
-| (t ≃ u)  := set.finite.union t.symbols_finite u.symbols_finite
-| (p ⟶ q)   := set.finite.union p.fn_symbols_finite q.fn_symbols_finite
-| (∼p)      := p.fn_symbols_finite
-| (∀.p)     := p.fn_symbols_finite
-
-lemma fn_symbols'_finite (p : formula L) (n : ℕ) : (p.fn_symbols' n).finite :=
-by { have : p.fn_symbols' n = (λ f : L.fn n, (⟨n, f⟩ : Σ n, L.fn n))⁻¹' p.fn_symbols, { refl },
-     rw this, refine set.finite.preimage (λ f, by simp) p.fn_symbols_finite  }
-
-lemma pr_symbols_finite : ∀ p : formula L, p.pr_symbols.finite
-| ⊤         := by simp
-| (app r v) := by simp
-| (t ≃ u)  := by simp
-| (p ⟶ q)   := set.finite.union p.pr_symbols_finite q.pr_symbols_finite
-| (∼p)      := p.pr_symbols_finite
-| (∀.p)     := p.pr_symbols_finite
-
-lemma pr_symbols'_finite (p : formula L) (n : ℕ) : (p.pr_symbols' n).finite :=
-by { have : p.pr_symbols' n = (λ r : L.pr n, (⟨n, r⟩ : Σ n, L.pr n))⁻¹' p.pr_symbols, { refl },
-     rw this, refine set.finite.preimage (λ r, by simp) p.pr_symbols_finite  }
-
-inductive subformula : formula L → formula L → Prop
-| neg    : ∀ {p}, subformula p (∼p)
-| implyl : ∀ {p q}, subformula p (p ⟶ q)
-| implyr : ∀ {p q}, subformula q (p ⟶ q)
-| fal    : ∀ {p}, subformula p (∀.p)
-
-@[simp] def complexity : formula L → ℕ
-| ⊤         := 0
-| (app r v) := 0
-| (t ≃ u)  := 0
-| (∼p)      := p.complexity + 1
-| (p ⟶ q)  := max p.complexity q.complexity + 1
-| (∀.p)     := p.complexity + 1
-
-instance : wf_lt (formula L) :=
-{ prelt := subformula,
-  wt := complexity,
-  mono' := λ a b h, by { induction h; try { simp },
-  case implyl : p q { exact nat.lt_succ_iff.mpr (le_max_left p.complexity q.complexity) },
-  case implyr : p q { exact nat.lt_succ_iff.mpr (le_max_right p.complexity q.complexity) } } }
-
-@[simp] lemma lt_app {p : formula L} {n} {r : L.pr n} {v} : ¬p < app r v :=
-by { simp [wf_lt.lt_iff], intros p h, rcases h }
-
-@[simp] lemma le_app {p : formula L} {n} {r : L.pr n} {v} : p ≤ app r v ↔ p = app r v := by simp[le_iff_lt_or_eq]
-
-@[simp] lemma lt_equal {p : formula L} {t u : term L} : ¬p < (t ≃ u) :=
-by { simp [wf_lt.lt_iff], intros p h, rcases h }
-
-@[simp] lemma le_equal {p : formula L} {t u : term L} : p ≤ (t ≃ u) ↔ p = (t ≃ u) := by simp[le_iff_lt_or_eq]
-
-@[simp] lemma lt_verum {p : formula L} : ¬p < ⊤ :=
-by { simp [wf_lt.lt_iff], intros p h, rcases h }
-
-@[simp] lemma le_verum {p : formula L} : p ≤ ⊤ ↔ p = ⊤ := by simp[le_iff_lt_or_eq]
-
-@[simp] lemma lt_imply {p q r : formula L} :
-  p < q ⟶ r ↔ p ≤ q ∨ p ≤ r :=
-begin
-  simp [wf_lt.lt_iff], split,
-  { rintros ⟨p', h, le⟩, rcases h, { exact or.inl le }, { exact or.inr le } },
-  rintros (le | le),
-  { refine ⟨q, subformula.implyl, le⟩ }, { refine ⟨r, subformula.implyr, le⟩ }
-end
-
-@[simp] lemma lt_neg {p q : formula L} :
-  p < ∼q ↔ p ≤ q :=
-begin
-  simp [wf_lt.lt_iff], split,
-  { rintros ⟨p', h, le⟩, rcases h, exact le },
-  rintros le,
-  { refine ⟨q, subformula.neg, le⟩ }
-end
-
-@[simp] lemma lt_fal {p q : formula L} :
-  p < ∀.q ↔ p ≤ q :=
-begin
-  simp [wf_lt.lt_iff], split,
-  { rintros ⟨p', h, le⟩, rcases h, exact le },
-  rintros le,
-  { refine ⟨q, subformula.fal, le⟩ }
-end
-
-lemma rew_inversion_of_le_rew {p q : formula L} {s} (le : p ≤ q.rew s) : ∃ (p' ≤ q) (k : ℕ), p = p'.rew (s^k) :=
-begin
-  induction q generalizing p s; try { simp* },
-  case app : n r v { simp at le, rcases le with rfl, refine ⟨0, by simp⟩ },
-  case equal : t u { simp at le, rcases le with rfl, refine ⟨0, by simp⟩ },
-  case verum { simp at le, exact le },
-  case imply : q₁ q₂ IH₁ IH₂
-  { rcases le_iff_lt_or_eq.mp le with (lt | rfl),
-    { simp at lt, rcases lt with (le | le),
-      { rcases IH₁ le with ⟨p', le_p', k, rfl⟩, refine ⟨p', le_trans le_p' (le_of_lt (by simp)), k, by refl⟩ },
-      { rcases IH₂ le with ⟨p', le_p', k, rfl⟩, refine ⟨p', le_trans le_p' (le_of_lt (by simp)), k, by refl⟩ } },
-    { refine ⟨q₁ ⟶ q₂, by simp, 0, by simp⟩ } },
-  case neg : q IH
-  { rcases le_iff_lt_or_eq.mp le with (lt | rfl),
-    { simp at lt, rcases IH lt with ⟨p', le_p', k, rfl⟩, refine ⟨p', le_trans le_p' (le_of_lt (by simp)), k, by refl⟩ },
-    { refine ⟨∼q, by refl, 0, by refl⟩ } },
-  case fal : q IH
-  { rcases le_iff_lt_or_eq.mp le with (lt | rfl),
-    { simp at lt, rcases IH lt with ⟨p', le_p', k, rfl⟩, 
-      refine ⟨p', le_trans le_p' (le_of_lt (by simp)), k + 1, by simp[rewriting_sf_itr.pow_add, add_comm 1]⟩ },
-    { refine ⟨∀.q, by refl, 0, by simp⟩ } }
-end
-
-lemma fn_symbols_ss_of_le {p q : formula L} (h : p ≤ q) : p.fn_symbols ⊆ q.fn_symbols :=
-by { induction h; try { simp },
-     case refl { refl },
-     case trans : p q r _ _ IH_pq IH_qr { exact set.subset.trans IH_pq IH_qr },
-     case of_prelt : p q prelt { induction prelt; try { simp } } }
-
-lemma pr_symbols_ss_of_le {p q : formula L} (h : p ≤ q) : p.pr_symbols ⊆ q.pr_symbols :=
-by { induction h; try { simp },
-     case refl { refl },
-     case trans : p q r _ _ IH_pq IH_qr { exact set.subset.trans IH_pq IH_qr },
-     case of_prelt : p q prelt { induction prelt; try { simp } } }
-
-inductive subterm : term L → formula L → Prop
-| app    : ∀ {n} (r : L.pr n) (v : finitary (term L) n) (i), subterm (v i) (app r v)
-| equall : ∀ {t u : term L}, subterm t (t ≃ u)
-| equalr : ∀ {t u : term L}, subterm u (t ≃ u)
-
-instance : has_mem (term L) (formula L) := ⟨λ t p, ∃ (t' ≥ t) (p' ≤ p), subterm t' p'⟩
-
-lemma mem_def {t : term L} {p : formula L} : t ∈ p ↔ ∃ (t' ≥ t) (p' ≤ p), subterm t' p' := by refl
-
-@[simp] lemma mem_equall (t u : term L) : t ∈ (t ≃ u : formula L) := ⟨t, by simp, t ≃ u, by simp, subterm.equall⟩ 
-
-@[simp] lemma mem_equalr (t u : term L) : u ∈ (t ≃ u : formula L) := ⟨u, by simp, t ≃ u, by simp, subterm.equalr⟩ 
-
-lemma mem_of_formula_le_mem {t : term L} {p q : formula L} : t ∈ p → p ≤ q → t ∈ q :=
-by { rintros ⟨t', ht', p', hp', sb⟩ le, refine ⟨t', ht', p', (le_trans hp' le), sb⟩ }
-
-lemma mem_of_term_le_mem {t u : term L} {p : formula L} : u ∈ p → t ≤ u → t ∈ p :=
-by { rintros ⟨t', ht', p', hp', sb⟩ le, refine ⟨t', le_trans le ht', p', hp', sb⟩ }
-
-@[simp] lemma mem_app {t : term L} {n} {r : L.pr n} {v : finitary (term L) n} :
-  t ∈ app r v ↔ ∃ i, t ≤ v i :=
-⟨by { rintros ⟨t', ht', p', hp', sb⟩,
-      have hp' : p' = app r v ∨ p' < app r v, exact eq_or_lt_of_le hp', simp at hp',
-      rcases hp' with rfl, cases sb with i, refine ⟨_, ht'⟩ },
- by { rintros ⟨i, le⟩, refine mem_of_term_le_mem ⟨v i, by simp, app r v, by simp, subterm.app r v i⟩ le }⟩
-
-@[simp] lemma mem_equal {s t u : term L} :
-  s ∈ (t ≃ u : formula L) ↔ s ≤ t ∨ s ≤ u :=
-⟨by { rintros ⟨t', ht', p', hp', sb⟩,
-      have hp' : p' = (t ≃ u) ∨ p' < (t ≃ u), exact eq_or_lt_of_le hp', simp at hp',
-      rcases hp' with rfl, cases sb, { exact or.inl ht' }, { exact or.inr ht' } },
- by { rintros (le | le),
-      { refine mem_of_term_le_mem ⟨t, by simp, t ≃ u, by simp, subterm.equall⟩ le },
-      { refine mem_of_term_le_mem ⟨u, by simp, t ≃ u, by simp, subterm.equalr⟩ le } }⟩
-
-@[simp] lemma mem_verum {t : term L} :
-  ¬t ∈ (⊤ : formula L) :=
-by { rintros ⟨t', ht', p', hp', sb⟩, 
-      have hp' : p' = ⊤ ∨ p' < ⊤, exact eq_or_lt_of_le hp', simp at hp',
-      rcases hp' with rfl, rcases sb }
-
-@[simp] lemma mem_imply {t : term L} {p q : formula L} :
-  t ∈ p ⟶ q ↔ t ∈ p ∨ t ∈ q :=
-⟨by { rintros ⟨t', ht', p', hp', sb⟩, 
-      have hp' : p' = p ⟶ q ∨ p' < p ⟶ q, exact eq_or_lt_of_le hp', simp at hp',
-      rcases hp' with (rfl | (hp' | hp')),
-      { rcases sb }, { refine or.inl ⟨t', ht', p', hp', sb⟩ }, { refine or.inr ⟨t', ht', p', hp', sb⟩ }  },
- by { rintros (h | h); refine mem_of_formula_le_mem h (le_of_lt (by simp)) }⟩
-
-@[simp] lemma mem_neg {t : term L} {p : formula L} :
-  t ∈ ∼p ↔ t ∈ p :=
-⟨by { rintros ⟨t', ht', p', hp', sb⟩, 
-      have hp' : p' = ∼p ∨ p' < ∼p, exact eq_or_lt_of_le hp', simp at hp',
-      rcases hp' with (rfl | hp'),
-      { rcases sb }, { refine ⟨t', ht', p', hp', sb⟩ }  },
- by { rintros h, refine mem_of_formula_le_mem h (le_of_lt (by simp)) }⟩
-
-@[simp] lemma mem_fal {t : term L} {p : formula L} :
-  t ∈ ∀.p ↔ t ∈ p :=
-⟨by { rintros ⟨t', ht', p', hp', sb⟩, 
-      have hp' : p' = ∀.p ∨ p' < ∀.p, exact eq_or_lt_of_le hp', simp at hp',
-      rcases hp' with (rfl | hp'),
-      { rcases sb }, { refine ⟨t', ht', p', hp', sb⟩ }  },
- by { rintros h, refine mem_of_formula_le_mem h (le_of_lt (by simp)) }⟩
-
-@[simp] lemma mem_ex {t : term L} {p : formula L} :
-  t ∈ ∃. p ↔ t ∈ p := by simp[ex_eq]
-
-lemma rew_inversion_or_le_of_mem_rew {t : term L} {p : formula L} {s} (mem : t ∈ p.rew s) :
- (∃ (t' : term L) (mem : t' ∈ p) (k : ℕ), t = t'.rew (s^k)) ∨ (∃ (k n : ℕ), t ≤ (s^k) n) :=
-begin
-  induction p generalizing t s,
-  case app : n r v
-  { simp at mem, rcases mem with ⟨i, le⟩,
-    rcases term.rew_inversion_or_le_of_le_rew le with (⟨t', le_t', rfl⟩ | h),
-    { refine or.inl ⟨t', by { simp; exact ⟨i, le_t'⟩ }, 0, rfl⟩ },
-    { exact or.inr ⟨0, h⟩ } },
-  case equal : u₁ u₂
-  { simp at mem, rcases mem with (le | le),
-    { rcases term.rew_inversion_or_le_of_le_rew le with (⟨t', le_t', rfl⟩ | h),
-      { refine or.inl ⟨t', by simp[le_t'], 0, rfl⟩ },
-      { exact or.inr ⟨0, h⟩ } },
-    { rcases term.rew_inversion_or_le_of_le_rew le with (⟨t', le_t', rfl⟩ | h),
-      { refine or.inl ⟨t', by simp[le_t'], 0, rfl⟩ },
-      { exact or.inr ⟨0, h⟩ } } },
-  case verum { simp at mem, contradiction },
-  case imply : p q IH_p IH_q
-  { simp at mem, rcases mem with (mem | mem),
-    { rcases IH_p mem with (⟨t', mem', k, rfl⟩ | h),
-      { refine or.inl ⟨t', by simp[mem'], k, rfl⟩ }, { exact or.inr h } },
-    { rcases IH_q mem with (⟨t', mem', k, rfl⟩ | h),
-      { refine or.inl ⟨t', by simp[mem'], k, rfl⟩ }, { exact or.inr h } } },
-  case neg : p IH
-  { simp at mem,
-    { rcases IH mem with (⟨t', mem', k, rfl⟩ | h),
-      { refine or.inl ⟨t', by simp[mem'], k, rfl⟩ }, { exact or.inr h } }, },
-  case fal : p IH
-  { simp at mem, rcases IH mem with (⟨t', mem', k, rfl⟩ | h),
-    { refine or.inl ⟨t', by simp[mem'], k + 1, by simp[rewriting_sf_itr.pow_add, add_comm 1]⟩ },
-    { rcases h with ⟨k, h⟩, simp[rewriting_sf_itr.pow_add, add_comm 1] at h,
-      refine or.inr ⟨k+1, h⟩ } }
-end
-
-lemma fn_symbols_ss_of_mem {t : term L} {p : formula L} (h : t ∈ p) : t.symbols ⊆ p.fn_symbols :=
-begin
-  have ss : ∀ {t : term L} {p : formula L}, subterm t p → t.symbols ⊆ p.fn_symbols,
-  { intros t p sub, induction sub; try { simp },
-    case app : n r v i { refine set.subset_Union _ i } },
-  rcases h with ⟨t', le_t, p', le_p, sub⟩,
-  have t_ss_t' : t.symbols ⊆ t'.symbols, from term.symbols_ss_of_le le_t,
-  have p'_ss_p : p'.fn_symbols ⊆ p.fn_symbols, from fn_symbols_ss_of_le le_p,
-  exact set.subset.trans (set.subset.trans t_ss_t' (ss sub)) p'_ss_p
-end
-
-lemma prelt_finite (p : formula L) : set.finite {q | subformula q p} :=
-begin
-  induction p,
-  case verum { have : {q : formula L | q.subformula ⊤} = ∅, { ext q, simp, intros h, rcases h }, simp[this] },
-  case app : n r v { have : {q : formula L | q.subformula (app r v)} = ∅, { ext q, simp, intros h, rcases h }, simp[this] },
-  case equal : t u { have : {q : formula L | q.subformula (t ≃ u)} = ∅, { ext q, simp, intros h, rcases h }, simp[this] },
-  case imply : p q { have : {r : formula L | r.subformula (p ⟶ q)} = {p, q},
-    { ext r, simp, split, { rintros h, rcases h; simp }, { rintros (rfl | rfl), exact subformula.implyl, exact subformula.implyr } },
-    simp[this] },
-  case neg : p IH
-  { have : {q : formula L | q.subformula (∼p)} = {p},
-    { ext q, simp, split, { intros h, rcases h, simp }, { rintros rfl, exact subformula.neg } },
-    simp[this] },
-  case fal : p IH
-  { have : {q : formula L | q.subformula (∀.p)} = {p},
-    { ext q, simp, split, { intros h, rcases h, simp }, { rintros rfl, exact subformula.fal } },
-    simp[this] }
-end
-
-lemma le_finite (p : formula L) : set.finite {q | q ≤ p} :=
-wf_lt.le_finite (show ∀ (a : formula L), {b : formula L | wf_lt.prelt b a}.finite, from prelt_finite) p
-
-lemma subterm_finite (p : formula L) : set.finite {t : term L | subterm t p} :=
-begin
-  induction p,
-  case verum { have : {t : term L | subterm t ⊤} = ∅, { ext t, simp, intros h, rcases h }, simp[this] },
-  case app : n r v
-  { have : {t : term L | subterm t (app r v)} = set.range v,
-    { ext t, simp, split,
-      { intros h, rcases h, simp }, { rintros ⟨i, rfl⟩, exact subterm.app r v i } },
-    simp[this, set.finite_range] },
-  case equal : t u
-  { have : {s : term L | subterm s (t ≃ u)} = {t, u},
-    { ext s, simp, split,
-      { intros h, rcases h; simp }, { rintros (rfl | rfl), exact subterm.equall, exact subterm.equalr } },
-    simp[this] },
-  case imply : p q
-  { have : {t : term L | subterm t (p ⟶ q)} = ∅, { ext r, simp, intros h, rcases h }, simp[this] },
-  case neg : p IH
-  { have : {t : term L | subterm t (∼p)} = ∅, { ext r, simp, intros h, rcases h }, simp[this] },
-  case fal : p IH
-  { have : {t : term L | subterm t (∀.p)} = ∅, { ext r, simp, intros h, rcases h }, simp[this] }
-end
-
-lemma mem_finite (p : formula L) : set.finite {t : term L | t ∈ p} :=
-begin
-  let s := ⋃ q ∈ {q | q ≤ p}, {t : term L | subterm t q},
-  let b := ⋃ t ∈ s, {u | u ≤ t},
-  have : {t : term L | t ∈ p} = b,
-  { ext t, simp[b, s, mem_def], split,
-    { rintros ⟨t', t_le_t', ⟨p', p'_le_p, t'_st_p'⟩⟩, refine ⟨p', p'_le_p, t', t'_st_p', t_le_t'⟩ },
-    { rintros ⟨p', p'_le_p, t', t'_st_p', t_le_t'⟩, exact ⟨t', t_le_t', ⟨p', p'_le_p, t'_st_p'⟩⟩ } },
-  simp[this],
-  have : s.finite, from set.finite.bUnion (le_finite p) (λ q h, subterm_finite q),
-  refine set.finite.bUnion this (λ u h, term.le_finite u),
-end
-
-@[simp] lemma formula.ite_pow (p : Prop) [decidable p] (q r : formula L) (k : ℕ) :
-  (ite p q r)^k = ite p (q^k) (r^k) :=
-by by_cases C : p; simp[C]
-
-class abberavation₁ (f : term L → formula L) :=
-(map_rew : ∀ s t, (f t).rew s = f (t.rew s))
-(arity : ∀ t, (f t).arity = t.arity)
-
-attribute [simp] abberavation₁.map_rew abberavation₁.arity
-
-class abberavation₂ (f : term L → term L → formula L) :=
-(map_rew : ∀ s t u, (f t u).rew s = f (t.rew s) (u.rew s))
-(arity : ∀ t u, (f t u).arity = max t.arity u.arity)
-
-attribute [simp] abberavation₂.map_rew abberavation₂.arity
-
-namespace abberavation₁
-variables (f : term L → formula L) [abberavation₁ f] (t : term L)
-
-@[simp] lemma map_pow (n : ℕ) : (f t)^n = f (t^n) := by simp[formula.pow_eq, term.pow_eq]
-
-lemma eq_rew : (f #0).rew (t ⌢ ı) = f t := by simp
-
-end abberavation₁
-
-namespace abberavation₂
-variables (f : term L → term L → formula L) [abberavation₂ f] (t u : term L)
-
-@[simp] lemma map_pow (n : ℕ) : (f t u)^n = f (t^n) (u^n) := by simp[formula.pow_eq, term.pow_eq]
-
-lemma eq_rew : f t u = (f #0 #1).rew (t ⌢ u ⌢ ı) := by simp
-
-end abberavation₂
-
-end formula
-
-namespace language
-
-class predicate (L : language.{u}) :=
-(fun_empty : ∀ n, is_empty (L.fn n))
-
-instance [predicate L] (n) : is_empty (L.fn n) := predicate.fun_empty n
-
-end language
+end push
+
+def pull' {m} : Π {n}, subformula L (m + 1) n → subformula L m (n + 1)
+| n verum          := ⊤
+| n (relation p v) := relation p (subterm.pull ∘ v)
+| n (equal t u)    := t.pull =' u.pull
+| n (imply p q)    := p.pull' ⟶ q.pull'
+| n (neg p)        := ∼p.pull'
+| n (fal p)        := ∀'p.pull'
+
+def pull : subformula L (m + 1) n →ₗ subformula L m (n + 1) :=
+{ to_fun := pull',
+  map_neg' := λ p, by refl,
+  map_imply' := λ p q, by refl,
+  map_and' := λ p q, by refl,
+  map_or' := λ p q, by refl,
+  map_top' := by refl,
+  map_bot' := by refl }
+
+section pull
+
+lemma pull_def (p : subformula L (m + 1) n) : pull p = pull' p := rfl
+
+@[simp] lemma pull_relation {p} (r : L.pr p) (v : finitary (subterm L (m + 1) n) p) :
+  pull (relation r v) = relation r (subterm.pull ∘ v) := by refl
+
+@[simp] lemma pull_equal (t u : subterm L (m + 1) n) :
+  pull (t =' u : subformula L (m + 1) n) = (t.pull =' u.pull) := by refl
+
+@[simp] lemma pull_fal (p : subformula L (m + 1) (n + 1)) :
+  pull (∀'p) = ∀'pull p := by refl
+
+@[simp] lemma pull_ex (p : subformula L (m + 1) (n + 1)) :
+  pull (∃'p) = ∃'pull p := by simp[ex_def]
+
+end pull
+
+def dummy : subformula L m n →ₗ subformula L m (n + 1) := pull.comp mlift
+
+section dummy
+
+@[simp] lemma dummy_relation {p} (r : L.pr p) (v : finitary (subterm L m n) p) :
+  dummy (relation r v) = relation r (subterm.dummy ∘ v) := by simp[dummy, subterm.dummy]
+
+@[simp] lemma dummy_equal (t u : subterm L m n) :
+  dummy (t =' u : subformula L m n) = (t.dummy =' u.dummy) := by simp[dummy, subterm.dummy]
+
+@[simp] lemma dummy_fal (p : subformula L m (n + 1)) : dummy (∀'p) = ∀'(dummy p) := by simp[dummy]
+
+@[simp] lemma dummy_ex (p : subformula L m (n + 1)) : dummy (∃'p) = ∃'(dummy p) := by simp[dummy]
+
+end dummy
+
+@[simp] lemma push_pull : ∀ {n} (p : subformula L m (n + 1)), p.push.pull = p
+| n verum          := by simp[top_eq]
+| n (relation p v) := by simp; funext x; simp
+| n (equal t u)    := by simp[equal_eq]
+| n (imply p q)    := by simp[imply_eq]; exact ⟨push_pull p, push_pull q⟩
+| n (neg p)        := by simp[neg_eq]; exact push_pull p
+| n (fal p)        := by simp[fal_eq]; exact push_pull p
+using_well_founded {rel_tac := λ _ _, `[exact ⟨_, measure_wf (λ x, x.2.complexity)⟩]}
+
+@[simp] lemma pull_push : ∀ {n} (p : subformula L (m + 1) n), p.pull.push = p
+| n verum          := by simp[top_eq]
+| n (relation p v) := by simp; funext x; simp
+| n (equal t u)    := by simp[equal_eq]
+| n (imply p q)    := by simp[imply_eq]; exact ⟨pull_push p, pull_push q⟩
+| n (neg p)        := by simp[neg_eq]; exact pull_push p
+| n (fal p)        := by simp[fal_eq]; exact pull_push p
+
+def qr {m} : Π {n}, subformula L m n → ℕ
+| n verum          := 0
+| n (relation r v) := 0
+| n (equal t u)    := 0
+| n (imply p q)    := max p.qr q.qr
+| n (neg p)        := p.qr
+| n (fal p)        := p.qr + 1
+
+def is_open {m n} (p : subformula L m n) : Prop := p.qr = 0
+
+section qr
+variables {m n}
+
+@[simp] lemma qr_top : (⊤ : subformula L m n).qr = 0 := rfl
+
+@[simp] lemma qr_bot : (⊥ : subformula L m n).qr = 0 := rfl
+
+@[simp] lemma qr_relation {p} (r : L.pr p) (v : finitary (subterm L m n) p) : (relation r v).qr = 0 := rfl
+
+@[simp] lemma qr_equal (t u : subterm L m n) : (t =' u : subformula L m n).qr = 0 := rfl
+
+@[simp] lemma qr_imply (p q : subformula L m n) : (p ⟶ q : subformula L m n).qr = max p.qr q.qr := rfl
+
+@[simp] lemma qr_and (p q : subformula L m n) : (p ⊓ q : subformula L m n).qr = max p.qr q.qr := rfl
+
+@[simp] lemma qr_or (p q : subformula L m n) : (p ⊔ q : subformula L m n).qr = max p.qr q.qr := rfl
+
+@[simp] lemma qr_iff (p q : subformula L m n) : (p ⟷ q : subformula L m n).qr = max p.qr q.qr := by simp[lrarrow_def, max_comm]
+
+@[simp] lemma qr_neg (p : subformula L m n) : (∼p).qr = p.qr := rfl
+
+@[simp] lemma qr_fal (p : subformula L m (n + 1)) : (∀'p).qr = p.qr + 1 := rfl
+
+@[simp] lemma qr_ex (p : subformula L m (n + 1)) : (∃'p).qr = p.qr + 1 := rfl
+
+end qr
+
+end subformula
+
+namespace preTheory
+variables {L} {m : ℕ} (T U : preTheory L m)
+
+def mlift : preTheory L (m + 1) := subformula.mlift '' T
+
+lemma mlift_insert (p : formula L m) : (insert p T).mlift = insert p.mlift T.mlift :=
+by simp[mlift, set.image_insert_eq]
+
+end preTheory
 
 end fol
